src/theory/bir/bir_programSyntax.sml
@@ -253,6 +253,8 @@ val (bst_environ_tm,  mk_bst_environ, dest_bst_environ, is_bst_environ)  = synta
 val (bst_pc_tm,  mk_bst_pc, dest_bst_pc, is_bst_pc)  = syntax_fns1 "bir_state_t_bst_pc";
 
 
+val (bir_state_init_tm,  mk_bir_state_init, dest_bir_state_init, is_bir_state_init)  = syntax_fns1 "bir_state_init";
+
 val (bir_state_is_terminated_tm,  mk_bir_state_is_terminated, dest_bir_state_is_terminated, is_bir_state_is_terminated)  = syntax_fns1 "bir_state_is_terminated";
 
 
