src/theory/bir/bir_envScript.sml
@@ -17,708 +17,438 @@ val bir_var_eq_EXPAND = store_thm ("bir_var_eq_EXPAND",
                         (bir_var_type v1 = bir_var_type v2)``,
 
 Cases >> Cases >>
-SIMP_TAC std_ss [bir_var_type_def, bir_var_name_def, bir_var_t_11]
-);
+SIMP_TAC std_ss [bir_var_type_def, bir_var_name_def, bir_var_t_11])
 
 
-val _ = Datatype `bir_var_environment_t =
-   BEnv (string -> (bir_val_k_t))`;
-val bir_var_environment_t_11 =
-  DB.fetch "-" "bir_var_environment_t_11";
-
-(* Empty environment *)
-(* TODO: What now? *)
-(*
-val bir_empty_env_def = Define `bir_empty_env = BEnv FEMPTY`
-*)
-(* Deprecated
-val bir_is_well_typed_env_def = Define `
-  (bir_is_well_typed_env (BEnv m) <=> FEVERY (\ (_, (ty, vo)).
-     (case vo of NONE => T | SOME v => (SOME ty = type_of_bir_val v))) m)`;
-*)
-(* Deprecated
-val bir_is_well_typed_env_empty = store_thm ("bir_is_well_typed_env_empty",
-  ``bir_is_well_typed_env bir_empty_env``,
-SIMP_TAC std_ss [bir_is_well_typed_env_def, bir_empty_env_def, FEVERY_FEMPTY]);
-*)
+val _ = Datatype `bir_var_environment_t = BEnv (string -> (bir_val_t option))`;
+val bir_var_environment_t_11 = DB.fetch "-" "bir_var_environment_t_11";
 
 val bir_env_lookup_def = Define `
   (bir_env_lookup varname (BEnv env) = env varname)`;
 
 val bir_env_update_def = Define `
-  (bir_env_update varname vo vartype (BEnv env) =
-    if (vartype <> type_of_bir_kval vo)
-    then NONE
-    else SOME (BEnv ((varname =+ vo) env))
-  )`;
+  (bir_env_update varname v (BEnv env) = BEnv ((varname =+ SOME v) env))`;
 
 val bir_env_lookup_UPDATE = store_thm ("bir_env_lookup_UPDATE",
-  ``!vn vn' vo env.
-    bir_env_lookup vn (BEnv ((vn' =+ vo) env)) =
-     (if (vn' = vn)
-      then vo
-      else bir_env_lookup vn (BEnv env))``,
-
-SIMP_TAC std_ss [bir_env_lookup_def, UPDATE_def]
-);
-
+``bir_env_lookup vn (BEnv ((vn' =+ vo) env)) =
+   (if (vn' = vn) then vo else bir_env_lookup vn (BEnv env))``,
+SIMP_TAC std_ss [bir_env_lookup_def, APPLY_UPDATE_THM]);
 
 val bir_env_lookup_type_def = Define `
-  bir_env_lookup_type var_name env =
-    type_of_bir_kval (bir_env_lookup var_name env)`;
+  bir_env_lookup_type var_name env = OPTION_MAP type_of_bir_val (bir_env_lookup var_name env)`;
 
 
 val bir_env_check_type_def = Define `
   bir_env_check_type var env =
-    (bir_env_lookup_type (bir_var_name var) env =
-      bir_var_type var
-    )`;
+    (bir_env_lookup_type (bir_var_name var) env = SOME (bir_var_type var))`;
 
-(* Note design choice: BVal_Unknown is returned upon explicit type
- * disagreement between stored and looked-up variable. *)
-val bir_env_read_def = Define `bir_env_read v env =
-  if (bir_env_check_type v env)
-  then BVal_Known (bir_env_lookup (bir_var_name v) env)
-  else BVal_Unknown`;
+
+val bir_env_read_def = Define `bir_env_read var env =
+  if (bir_env_check_type var env) then
+    (bir_env_lookup (bir_var_name var) env)
+  else
+    NONE`;
 
 
 val bir_env_read_UPDATE = store_thm ("bir_env_read_UPDATE",
-  ``!v vn vo env.
-    bir_env_read v (BEnv ((vn =+ vo) env)) =
-      (if (bir_var_name v = vn)
-       then (if (type_of_bir_kval vo = bir_var_type v)
-             then BVal_Known vo
-             else BVal_Unknown
-            )
-       else bir_env_read v (BEnv env)
-      )``,
+``bir_env_read var (BEnv ((vn =+ vo) env)) =
+   (if (bir_var_name var = vn) then
+      (if (OPTION_MAP type_of_bir_val vo) = SOME (bir_var_type var) then
+         vo
+       else
+         NONE)
+    else bir_env_read var (BEnv env))``,
 
-REPEAT STRIP_TAC >>
-SIMP_TAC std_ss [bir_env_read_def, bir_env_lookup_UPDATE] >>
-Cases_on `bir_var_name v = vn` >> (
-  FULL_SIMP_TAC std_ss [type_of_bir_kval_def,
-			bir_env_check_type_def,
-			bir_env_lookup_type_def,
-                        bir_env_lookup_def,
-			combinTheory.UPDATE_APPLY]
-)
-);
+SIMP_TAC std_ss [bir_env_read_def, bir_env_lookup_UPDATE,
+      bir_env_check_type_def, bir_env_lookup_type_def] >>
+Cases_on `bir_var_name var = vn` >> ASM_SIMP_TAC std_ss []);
 
-(* Note: Gains a new antecedent from no longer having type in the
- * returning tuple. *)
-val bir_env_read_NEQ_UNKNOWN =
-  store_thm ("bir_env_read_NEQ_UNKNOWN",
-  ``!var env v.
-    (type_of_bir_kval v = bir_var_type var) ==>
-    ((bir_env_read var env = BVal_Known v) <=>
-     (bir_env_lookup (bir_var_name var) env =
-        v
-     )
-    )``,
+val bir_env_write_def = Define `bir_env_write var va env =
+	 if (bir_env_check_type var env) /\ ((bir_var_type var) = (type_of_bir_val va)) then
+	   SOME (bir_env_update (bir_var_name var) va env)
+	 else
+	   NONE
+`;
 
-REPEAT STRIP_TAC >>
-SIMP_TAC std_ss [bir_env_read_def,
-                 bir_env_check_type_def,
-                 bir_env_lookup_type_def] >>
-REPEAT CASE_TAC >>
-METIS_TAC []
-);
+(* ===================== *)
 
-val bir_env_write_def = Define `bir_env_write v va env =
-  if (bir_env_check_type v env)
-  then bir_env_update (bir_var_name v) va (bir_var_type v) env
-  else NONE`;
-
-
-val bir_env_write_WrongVal = store_thm ("bir_env_write_WrongVal",
-  ``!v va env.
-    (type_of_bir_kval va <> bir_var_type v) ==>
-    (bir_env_write v va env = NONE)``,
+val bir_env_write_different_type = store_thm ("bir_env_write_different_type",
+  ``!v va env. (type_of_bir_val va <> bir_var_type v) ==>
+               (bir_env_write v va env = NONE)``,
 
 REPEAT GEN_TAC >> Cases_on `env` >>
-SIMP_TAC std_ss [bir_env_write_def,
-                 bir_env_check_type_def,
-                 bir_env_lookup_type_def, 
-                 bir_env_update_def]
+SIMP_TAC std_ss [bir_env_write_def, bir_env_update_def]
 );
 
-(* Deprecated...
-val bir_env_update_is_well_typed_env =
-  store_thm ("bir_env_update_is_well_typed_env",
-  ``!env env' varname vo ty.
-      (bir_is_well_typed_env env /\
-      (bir_env_update varname vo ty env = SOME env')) ==>
-      bir_is_well_typed_env env'``,
-
-Cases >>
-SIMP_TAC std_ss [bir_env_update_def, bir_is_well_typed_env_def] >>
-REPEAT STRIP_TAC >>
-ConseqConv.CONSEQ_REWRITE_TAC ([FEVERY_STRENGTHEN_THM], [], []) >>
-ASM_SIMP_TAC std_ss [] >>
-Cases_on `vo` >> (
-  FULL_SIMP_TAC std_ss []
-)
-);
-*)
-
-(* Deprecated...
-val bir_env_write_is_well_typed_env = store_thm ("bir_env_write_is_well_typed_env",
-``!env env' v va.
-    (bir_is_well_typed_env env /\
-    (bir_env_write v va env = SOME env')) ==>
-    bir_is_well_typed_env env'``,
-
-SIMP_TAC std_ss [bir_env_write_def] >>
-METIS_TAC[bir_env_update_is_well_typed_env]
-);
-*)
-
-(* Deprecated...
-val bir_is_well_typed_env_lookup =
-  store_thm ("bir_is_well_typed_env_lookup",
-  ``!env vn ty v. bir_is_well_typed_env env ==>
-                  (bir_env_lookup vn env = SOME (ty, SOME v)) ==>
-                  (type_of_bir_val v = SOME ty)``,
-
-Cases >> SIMP_TAC std_ss [bir_is_well_typed_env_def] >>
-rename1 `BEnv f` >>
-SIMP_TAC (std_ss++QI_ss) [bir_env_lookup_def, FEVERY_ALL_FLOOKUP] >>
-REPEAT STRIP_TAC >>
-Q.PAT_X_ASSUM `!k. _` (MP_TAC o Q.SPEC `vn`) >>
-ASM_SIMP_TAC std_ss []
-);
-*)
-
-(* Old name: bir_is_well_typed_env_read *)
-
-val bir_env_read_type =
-  store_thm ("bir_env_read_type",
-  ``!env v ty r.
-      (bir_env_read v env = r) ==>
-      (r <> BVal_Unknown) ==>
-      (type_of_bir_val r = SOME (bir_var_type v))``,
-
-SIMP_TAC std_ss [bir_env_read_def] >>
-REPEAT GEN_TAC >>
-REPEAT CASE_TAC >>
-FULL_SIMP_TAC std_ss [type_of_bir_val_def,
-                      bir_env_check_type_def,
-                      bir_env_lookup_type_def]
-);
-
-
-val bir_env_read_EQ_Unknown = store_thm ("bir_env_read_EQ_Unknown",
-  ``!v env.
-        (bir_env_read v env = BVal_Unknown) <=>
-          (!kv.
-            (type_of_bir_kval kv = bir_var_type v) ==>
-            (bir_env_lookup (bir_var_name v) env <>
-              kv
-            )
-          )``,
-
-REPEAT GEN_TAC >>
-SIMP_TAC std_ss [bir_env_read_def] >>
-REPEAT CASE_TAC >> (
-  FULL_SIMP_TAC std_ss [bir_env_lookup_type_def,
-			bir_env_check_type_def]
-)
-);
-(*
-(* All varnames are bound in a total map, so... *)
-val bir_env_varname_is_bound_def = Define `
-  (bir_env_varname_is_bound (BEnv env) var = (var IN FDOM env))`;
-
-val bir_env_varname_is_bound_ALT_DEF =
-  store_thm ("bir_env_varname_is_bound_ALT_DEF",
-  ``!var env.
-      bir_env_varname_is_bound env var <=>
-        IS_SOME (bir_env_lookup_type var env)``,
-
-Cases_on `env` >> (
-  SIMP_TAC (std_ss++boolSimps.LIFT_COND_ss)
-           [bir_env_varname_is_bound_def,
-            bir_env_lookup_type_def, bir_env_lookup_def,
-            FLOOKUP_DEF]
-)
-);
-
-val bir_env_varname_is_bound_ALT2_DEF =
-  store_thm ("bir_env_varname_is_bound_ALT2_DEF",
-  ``!var env.
-      bir_env_varname_is_bound env var <=>
-        IS_SOME (bir_env_lookup var env)``,
-
-SIMP_TAC std_ss [bir_env_varname_is_bound_ALT_DEF,
-                 bir_env_lookup_type_def,
-                 optionTheory.IS_SOME_MAP]
-);
-
-
-val bir_env_var_is_declared_def = Define `
-  (bir_env_var_is_declared env v <=>
-  (bir_env_lookup_type (bir_var_name v) env = SOME (bir_var_type v)))`;
-
-(* This duplication is kept deliberately, because despite the same
- * semantics, the intention of what you want to express is
- * different *)
-val bir_env_var_is_declared_DEF_bir_env_check_type =
-  store_thm ("bir_env_var_is_declared_ALT_DEF",
-  ``bir_env_var_is_declared env v = bir_env_check_type v env``,
-SIMP_TAC std_ss [bir_env_check_type_def,
-                 bir_env_var_is_declared_def]
-);
-*)
-
-(* Old name: bir_env_var_is_initialised *)
-val bir_env_var_is_well_typed_def = Define `
-  (bir_env_var_is_well_typed env var <=>
-    (?kv.
-      (bir_env_lookup (bir_var_name var) env = kv) /\
-      (type_of_bir_kval kv = bir_var_type var)
-    )
-  )`;
-(* No more declaration...
-val bir_env_var_is_initialised_weaken =
-  store_thm ("bir_env_var_is_initialised_weaken",
-  ``!v env.
-      bir_env_var_is_initialised env v ==>
-      bir_env_var_is_declared env v``,
-
-Cases >> SIMP_TAC std_ss [bir_env_var_is_initialised_def, bir_env_var_is_declared_def,
-  GSYM LEFT_FORALL_IMP_THM, bir_env_lookup_type_def]);
-*)
-(* No more declaration...
-val bir_env_var_is_declared_weaken =
-  store_thm ("bir_env_var_is_declared_weaken",
-  ``!v env.
-      bir_env_var_is_declared env v ==>
-      bir_env_varname_is_bound env (bir_var_name v)``,
-
-Cases >> SIMP_TAC std_ss [bir_env_var_is_declared_def,
-  GSYM LEFT_FORALL_IMP_THM, bir_env_varname_is_bound_ALT_DEF,
-  bir_var_name_def]);
-*)
-(* TODO: Remove now? *)
-val _ = Datatype `bir_env_cond_t =
-  | BEnvCond_var_well_typed bir_var_t`;
-
-val bir_env_cond_eval_def = Define `
-  (bir_env_cond_eval env (BEnvCond_var_well_typed v) <=>
-    bir_env_var_is_well_typed env v)`;
-
-
-val bir_env_order_def = Define `
-  (bir_env_order env1 env2) <=>
-    !vn. (
-(*
-     (* new vars can be added and initialised, but only of the
-      * correct type *)
-     (!ty v. (bir_env_lookup vn env1 = NONE) ==>
-             (bir_env_lookup vn env2 = SOME (ty, SOME v)) ==>
-             (type_of_bir_val v = SOME ty)
-     ) /\
-
-     (* existing vars can be initialised with the right type *)
-     (!ty. (bir_env_lookup vn env1 = SOME (ty, NONE)) ==>
-           (?vo. (bir_env_lookup vn env2 = SOME (ty, vo)) /\
-                 (!v. (vo = SOME v) ==>
-                      (type_of_bir_val v = SOME ty)
-                 )
-           )
-     ) /\
-*)
-     (* The value of existing vars can change, but their type
-      * cannot. *)
-     (!kv ty.
-       ((bir_env_lookup vn env1 = kv) /\
-        (type_of_bir_kval kv = ty)
-       )==>
-       (?kv'.
-         ((bir_env_lookup vn env2 = kv') /\
-          (type_of_bir_kval kv' = ty)
-         )
-       )
-     )
-   )`;
-
-
-val bir_env_order_REFL = store_thm ("bir_env_order_REFL",
-  ``!env. bir_env_order env env``,
-
-SIMP_TAC std_ss [bir_env_order_def]
-);
-
-
-val bir_env_order_TRANS = store_thm ("bir_env_order_TRANS",
-  ``!env1 env2 env3.
-      bir_env_order env1 env2 ==>
-      bir_env_order env2 env3 ==>
-      bir_env_order env1 env3``,
-
-METIS_TAC [bir_env_order_def]
-);
-
-(* All varnames are bound...
-val bir_env_varname_is_bound_ORDER =
-  store_thm ("bir_env_varname_is_bound_ORDER",
-  ``!env1 env2 v.
-      bir_env_order env1 env2 ==>
-      bir_env_varname_is_bound env1 v ==>
-      bir_env_varname_is_bound env2 v``,
-SIMP_TAC (std_ss++QI_ss) [bir_env_varname_is_bound_ALT_DEF, bir_env_order_def,
-  bir_env_lookup_type_def, optionTheory.IS_SOME_EXISTS] >>
-REPEAT STRIP_TAC >>
-rename1 `bir_env_lookup vn env1 = SOME (ty, vo)` >>
-Q.PAT_X_ASSUM `!vn. _` (MP_TAC o Q.SPEC `vn`) >>
-ASM_SIMP_TAC std_ss [] >>
-Cases_on `vo` >> (
-  SIMP_TAC std_ss [GSYM LEFT_FORALL_IMP_THM]
-));
-*)
-(* No more declare...
-val bir_env_var_is_declared_ORDER = store_thm ("bir_env_var_is_declared_ORDER",
-  ``!env1 env2 v. bir_env_order env1 env2 ==>
-                  bir_env_var_is_declared env1 v ==>
-                  bir_env_var_is_declared env2 v``,
-Cases_on `v` >>
-SIMP_TAC (std_ss++QI_ss) [bir_env_var_is_declared_def, bir_env_order_def,
-  bir_env_lookup_type_def] >>
-REPEAT STRIP_TAC >>
-rename1 `bir_env_lookup vn env1 = SOME (ty, vo)` >>
-Q.PAT_X_ASSUM `!vn. _` (MP_TAC o Q.SPEC `vn`) >>
-ASM_SIMP_TAC std_ss [] >>
-Cases_on `vo` >> (
-  SIMP_TAC std_ss [GSYM LEFT_FORALL_IMP_THM]
-));
-*)
-
-val bir_env_var_is_well_typed_ORDER =
-  store_thm ("bir_env_var_is_well_typed_ORDER",
-  ``!env1 env2 v.
-      bir_env_order env1 env2 ==>
-      bir_env_var_is_well_typed env1 v ==>
-      bir_env_var_is_well_typed env2 v``,
-
-SIMP_TAC std_ss [bir_env_var_is_well_typed_def,
-                 bir_env_order_def]
-);
-
-
-val bir_env_cond_eval_ORDER = store_thm ("bir_env_cond_eval_ORDER",
-  ``!env1 env2 c.
-      bir_env_order env1 env2 ==>
-      bir_env_cond_eval env1 c ==>
-      bir_env_cond_eval env2 c``,
-
-Cases_on `c` >> (
-  SIMP_TAC std_ss [bir_env_cond_eval_def] >>
-  METIS_TAC[bir_env_var_is_well_typed_ORDER]
-)
-);
-
-
-val bir_env_vars_are_well_typed_def = Define `
-  bir_env_vars_are_well_typed env vs <=>
-    (!v. v IN vs ==> bir_env_var_is_well_typed env v)`;
-
-val bir_env_vars_are_well_typed_EMPTY =
-  store_thm ("bir_env_vars_are_well_typed_EMPTY",
-  ``!env. bir_env_vars_are_well_typed env {}``,
-
-SIMP_TAC std_ss [bir_env_vars_are_well_typed_def, NOT_IN_EMPTY]
-);
-
-val bir_env_vars_are_well_typed_INSERT =
-  store_thm ("bir_env_vars_are_well_typed_INSERT",
-  ``!env v vs.
-      bir_env_vars_are_well_typed env (v INSERT vs) <=>
-        (bir_env_var_is_well_typed env v /\
-         bir_env_vars_are_well_typed env vs
-        )``,
-
-SIMP_TAC std_ss [bir_env_vars_are_well_typed_def, IN_INSERT] >>
-METIS_TAC []
-);
-
-val bir_env_vars_are_well_typed_UNION =
-  store_thm ("bir_env_vars_are_well_typed_UNION",
-  ``!env vs1 vs2.
-      bir_env_vars_are_well_typed env (vs1 UNION vs2) <=>
-        (bir_env_vars_are_well_typed env vs1 /\
-         bir_env_vars_are_well_typed env vs2) ``,
-
-SIMP_TAC std_ss [bir_env_vars_are_well_typed_def, IN_UNION] >>
-METIS_TAC []
-);
-
-val bir_env_vars_are_well_typed_SUBSET =
-  store_thm ("bir_env_vars_are_well_typed_SUBSET",
-  ``!env vs1 vs2.
-      bir_env_vars_are_well_typed env vs1 ==>
-      (vs2 SUBSET vs1) ==>
-      bir_env_vars_are_well_typed env vs2``,
-
-SIMP_TAC std_ss [bir_env_vars_are_well_typed_def, SUBSET_DEF] >>
-METIS_TAC []
-);
-
-
-val bir_env_vars_are_well_typed_ORDER =
-  store_thm ("bir_env_vars_are_well_typed_ORDER",
-  ``!env1 env2 vs.
-      bir_env_order env1 env2 ==>
-      bir_env_vars_are_well_typed env1 vs ==>
-      bir_env_vars_are_well_typed env2 vs``,
-
-SIMP_TAC std_ss [bir_env_vars_are_well_typed_def] >>
-METIS_TAC [bir_env_var_is_well_typed_ORDER]
-);
-
-(* Nonsensical with new changes?
-val bir_env_order_update = store_thm ("bir_env_order_update",
-``!env env' vn vo ty.
-    ~(bir_env_varname_is_bound env vn) /\
-    (bir_env_update vn vo ty env = SOME env') ==>
-    bir_env_order env env'``,
-
-Cases_on `env` >>
-SIMP_TAC std_ss [bir_env_update_def, bir_env_varname_is_bound_ALT_DEF] >>
-REPEAT STRIP_TAC >>
-FULL_SIMP_TAC (std_ss++boolSimps.LIFT_COND_ss++QI_ss) [
-  bir_env_lookup_type_def,
-  bir_env_lookup_def, bir_env_order_def,
-  FLOOKUP_UPDATE] >>
-METIS_TAC[]);
-*)
-
-val bir_env_order_write = store_thm ("bir_env_order_write",
+val bir_env_write_types = store_thm ("bir_env_write_types",
 ``!env env' v va.
     (bir_env_write v va env = SOME env') ==>
-    bir_env_order env env'``,
+    (bir_env_lookup_type (bir_var_name v) env = bir_env_lookup_type (bir_var_name v) env')``,
 
-Cases >>
-SIMP_TAC (std_ss++boolSimps.LIFT_COND_ss)
-         [bir_env_write_def, bir_env_update_def,
-          bir_env_order_def, bir_env_lookup_def,
-          bir_env_check_type_def, bir_env_lookup_type_def,
-          PULL_EXISTS] >>
-
-REPEAT STRIP_TAC >>
-Cases_on `bir_var_name v = vn` >> (
-  FULL_SIMP_TAC std_ss [combinTheory.UPDATE_APPLY]
-)
+SIMP_TAC std_ss [bir_env_write_def, bir_env_check_type_def] >>
+Cases_on `env` >>
+REWRITE_TAC [bir_env_update_def, bir_env_lookup_type_def, bir_env_lookup_type_def, bir_env_lookup_UPDATE] >>
+SIMP_TAC std_ss []
 );
 
-(* Deprecated...
-val bir_env_order_well_typed =
-  store_thm ("bir_env_order_well_typed",
-  ``!env env'.
-      bir_is_well_typed_env env ==>
-      bir_env_order env env' ==>
-      bir_is_well_typed_env env'``,
-
-Cases >> Cases >>
-rename1 `bir_env_order (BEnv env_f) (BEnv env_f')` >>
-SIMP_TAC (std_ss++QI_ss) [bir_is_well_typed_env_def,
-  bir_env_order_def, bir_env_lookup_def, PULL_FORALL, PULL_EXISTS,
-  FEVERY_ALL_FLOOKUP] >>
-REPEAT STRIP_TAC >>
-rename1 `FLOOKUP env_f' vn = SOME (ty, vo)` >>
-REPEAT (Q.PAT_X_ASSUM `!vn. _` (MP_TAC o Q.SPEC `vn`)) >>
-Cases_on `vo` >> SIMP_TAC std_ss [] >>
-rename1 `FLOOKUP env_f' vn = SOME (ty, SOME v')` >>
-ASM_SIMP_TAC std_ss [FORALL_AND_THM] >>
-Cases_on `FLOOKUP env_f vn` >- (
-  SIMP_TAC std_ss []
-) >>
-rename1 `FLOOKUP env_f vn = SOME (XXX)` >> Cases_on `XXX` >>
-rename1 `FLOOKUP env_f vn = SOME (ty', vo)` >>
-ASM_SIMP_TAC std_ss [] >>
-Cases_on `vo` >> SIMP_TAC std_ss []
-);
-*)
-
-(* Domains and subenvironment don't really makes sense with total
- * maps... *)
-(* Domains *)
-(*
-val bir_env_domain_def = Define `
-  bir_env_domain (BEnv env) = FDOM env`;
-
-val bir_env_domain_FINITE = store_thm ("bir_env_domain_FINITE",
-  ``!env. FINITE (bir_env_domain env)``,
-
-Cases >>
-SIMP_TAC std_ss [bir_env_domain_def, FDOM_FINITE]
-);
-
-
-val bir_env_domain_LOOKUP = store_thm ("bir_env_domain_LOOKUP",
-``!env vn. (vn IN (bir_env_domain env)) <=> IS_SOME (bir_env_lookup vn env)``,
-
-Cases >> GEN_TAC >>
-SIMP_TAC (std_ss++boolSimps.LIFT_COND_ss) [bir_env_domain_def, bir_env_lookup_def, FLOOKUP_DEF]);
-*)
-
-
-(* Subenvironments *)
-(*
-val bir_is_subenv_def = Define `bir_is_subenv (BEnv env1) (BEnv env2) <=> (env1 SUBMAP env2)`;
-
-val bir_is_subenv_EMPTY = store_thm ("bir_is_subenv_EMPTY",
-``!env. bir_is_subenv bir_empty_env env``,
-Cases >> SIMP_TAC std_ss [bir_is_subenv_def, bir_empty_env_def, SUBMAP_FEMPTY]);
-
-
-val bir_is_subenv_REFL = store_thm ("bir_is_subenv_REFL",
-  ``!env. bir_is_subenv env env``,
-Cases >> SIMP_TAC std_ss [bir_is_subenv_def, SUBMAP_REFL]);
-
-val bir_is_subenv_TRANS = store_thm ("bir_is_subenv_TRANS",
-  ``!env1 env2 env3. bir_is_subenv env1 env2 ==> bir_is_subenv env2 env3 ==> bir_is_subenv env1 env3``,
-REPEAT Cases >>
-SIMP_TAC std_ss [bir_is_subenv_def] >>
-METIS_TAC[SUBMAP_TRANS]);
-
-
-val bir_is_subenv_ANTISYM = store_thm ("bir_is_subenv_ANTISYM",
-  ``!env1 env2. (bir_is_subenv env1 env2 /\ bir_is_subenv env2 env1) <=> (env1 = env2)``,
-
-REPEAT Cases >>
-SIMP_TAC std_ss [bir_is_subenv_def, bir_var_environment_t_11] >>
-METIS_TAC[SUBMAP_ANTISYM]);
-
-
-val bir_is_subenv_domains = store_thm ("bir_is_subenv_domains",
-``!env1 env2. bir_is_subenv env1 env2 ==> (bir_env_domain env1 SUBSET bir_env_domain env2)``,
-REPEAT Cases >>
-SIMP_TAC std_ss [bir_is_subenv_def, bir_env_domain_def, SUBMAP_DEF, SUBSET_DEF]);
-
-
-
-val bir_is_subenv_LOOKUP = store_thm ("bir_is_subenv_LOOKUP",
-  ``!env1 env2 vn.
-       bir_is_subenv env1 env2 ==>
-       vn IN bir_env_domain env1 ==>
-       (bir_env_lookup vn env1 = bir_env_lookup vn env2)``,
-
-Cases >> Cases >> GEN_TAC >>
-SIMP_TAC std_ss [bir_is_subenv_def, bir_env_domain_def, bir_env_lookup_def,
-  SUBMAP_DEF, FLOOKUP_DEF])
-*)
-val bir_env_read_EQ_lookup_IMPL =
-  store_thm ("bir_env_read_EQ_lookup_IMPL",
-  ``!env1 env2 v.
-      (bir_env_lookup (bir_var_name v) env1 =
-        bir_env_lookup (bir_var_name v) env2) ==>
-      (bir_env_read v env1 = bir_env_read v env2)``,
-
-SIMP_TAC std_ss [bir_env_read_def,
-                 bir_env_check_type_def,
-                 bir_env_lookup_type_def]
-);
-
-(*
-val bir_is_subenv_READ = store_thm ("bir_is_subenv_READ",
-  ``!env1 env2 v.
-       bir_is_subenv env1 env2 ==>
-       (bir_var_name v) IN bir_env_domain env1 ==>
-       (bir_env_read v env1 = bir_env_read v env2)``,
+val bir_env_read_types = store_thm ("bir_env_read_types",
+  ``!env v ty r. (bir_env_read v env = r) ==>
+                 (r <> NONE) ==>
+                 (?va. (r = SOME va) /\ (type_of_bir_val va = bir_var_type v))``,
 
 SIMP_TAC std_ss [bir_env_read_def] >>
-METIS_TAC [bir_is_subenv_LOOKUP]);
+REPEAT GEN_TAC >>
+Cases_on `env` >>
+SIMP_TAC std_ss [bir_env_check_type_def, bir_env_lookup_type_def, bir_env_lookup_def] >>
+METIS_TAC[bir_env_check_type_def, bir_env_lookup_type_def]
+);
+
+(* ===================== *)
+
+
+val bir_env_read_EQ_lookup_IMPL = store_thm ("bir_env_read_EQ_lookup_IMPL",
+``!env1 env2 v.
+   (bir_env_lookup (bir_var_name v) env1 = bir_env_lookup (bir_var_name v) env2) ==>
+   (bir_env_read v env1 = bir_env_read v env2)``,
+SIMP_TAC std_ss [bir_env_read_def, bir_env_check_type_def, bir_env_lookup_type_def]);
+
+
+(* ===================== *)
+
+val _ = Datatype `bir_var_environment_typing_t = BEnvTy (string -> (bir_type_t option))`;
+
+val bir_envty_of_env_def = Define `bir_envty_of_env (BEnv env) =
+  BEnvTy ((OPTION_MAP type_of_bir_val) o env)
+`;
+
+val bir_env_satisfies_envty_def = Define `bir_env_satisfies_envty (BEnv env) (BEnvTy envty) =
+  !vn t. (envty vn = SOME t) ==> (?v. (env vn = SOME v) /\ (type_of_bir_val v = t))
+`;
+
+val bir_env_satisfies_envty_of_env = store_thm("bir_env_satisfies_envty_of_env", ``
+  !env. bir_env_satisfies_envty env (bir_envty_of_env env)
+``,
+  Cases_on `env` >>
+  SIMP_TAC std_ss [bir_env_satisfies_envty_def, bir_envty_of_env_def] >>
+  METIS_TAC[]
+);
+
+val bir_envty_includes_v_def = Define `bir_envty_includes_v (BEnvTy envty) v =
+  (envty (bir_var_name v) = SOME (bir_var_type v))
+`;
+
+val bir_envty_includes_vs_def = Define `bir_envty_includes_vs envty vs =
+  (!v. (v IN vs) ==> (bir_envty_includes_v envty v))
+`;
+
+val bir_v_in_envty_env_IMP = store_thm("bir_v_in_envty_env_IMP", ``
+  !envty env v. (bir_envty_includes_v envty v) ==>
+             (bir_env_satisfies_envty env envty) ==>
+             (?va. (bir_env_read v env = SOME va) /\ (type_of_bir_val va = bir_var_type v))
+``,
+  Cases_on `envty` >> Cases_on `env` >>
+  FULL_SIMP_TAC std_ss [bir_envty_includes_v_def, bir_env_satisfies_envty_def, bir_env_read_def, bir_env_check_type_def, bir_env_lookup_type_def, bir_env_lookup_def] >>
+  METIS_TAC []
+);
+
+val bir_vs_in_envty_env_IMP = store_thm("bir_vs_in_envty_env_IMP", ``
+  !envty env vs. (bir_envty_includes_vs envty vs) ==>
+             (bir_env_satisfies_envty env envty) ==>
+             !v. (v IN vs) ==>
+                 (?va. (bir_env_read v env = SOME va) /\ (type_of_bir_val va = bir_var_type v))
+``,
+  METIS_TAC [bir_envty_includes_vs_def, bir_v_in_envty_env_IMP]
+);
+
+
+val bir_vs_consistent_def = Define `bir_vs_consistent vs =
+  !v1 v2. (v1 IN vs) ==> (v2 IN vs) ==> ((bir_var_name v1) = (bir_var_name v2)) ==> (v1 = v2)
+`;
+
+val bir_envty_includes_vs_IMP_vs_consistent = store_thm("bir_envty_includes_vs_IMP_vs_consistent", ``
+  !envty vs. (bir_envty_includes_vs envty vs) ==>
+             (bir_vs_consistent vs)
+``,
+  Cases_on `envty` >>
+  SIMP_TAC std_ss [bir_envty_includes_vs_def, bir_envty_includes_v_def, bir_vs_consistent_def] >>
+  REPEAT STRIP_TAC >>
+  PAT_ASSUM ``!x. y`` (ASSUME_TAC o (Q.SPEC `v1`)) >>
+  PAT_ASSUM ``!x. y`` (ASSUME_TAC o (Q.SPEC `v2`)) >>
+  Cases_on `v1` >> Cases_on `v2` >>
+  SIMP_TAC std_ss [bir_var_eq_EXPAND, bir_var_name_def, bir_var_type_def] >>
+  Cases_on `s <> s'` >- (
+    METIS_TAC[bir_var_name_def]
+  ) >>
+  FULL_SIMP_TAC std_ss [bir_var_name_def, bir_var_type_def] >>
+  REV_FULL_SIMP_TAC std_ss []
+);
+
+val bir_envty_includes_vs_EMPTY = store_thm("bir_envty_includes_vs_EMPTY", ``
+  !envty. (bir_envty_includes_vs envty EMPTY)
+``,
+  Cases_on `envty` >>
+  SIMP_TAC std_ss [bir_envty_includes_vs_def, bir_envty_includes_v_def, NOT_IN_EMPTY]
+);
+
+val bir_envty_includes_vs_INSERT = store_thm("bir_envty_includes_vs_INSERT", ``
+  !envty v vs. (bir_envty_includes_vs envty (v INSERT vs)) <=>
+               ((bir_envty_includes_v envty v) /\ (bir_envty_includes_vs envty vs))
+``,
+  Cases_on `envty` >>
+  SIMP_TAC std_ss [bir_envty_includes_vs_def, IN_INSERT] >>
+  METIS_TAC[]
+);
+
+val bir_envty_includes_vs_UNION = store_thm("bir_envty_includes_vs_UNION", ``
+  !envty vs1 vs2. (bir_envty_includes_vs envty (vs1 UNION vs2)) <=>
+                  ((bir_envty_includes_vs envty vs1) /\ (bir_envty_includes_vs envty vs2))
+``,
+  Cases_on `envty` >>
+  SIMP_TAC std_ss [bir_envty_includes_vs_def, IN_UNION] >>
+  METIS_TAC[]
+);
+
+val bir_envty_includes_vs_SUBSET = store_thm("bir_envty_includes_vs_SUBSET", ``
+  !envty vs1 vs2. (bir_envty_includes_vs envty vs1) ==>
+                  (vs2 SUBSET vs1) ==>
+                  (bir_envty_includes_vs envty vs2)
+``,
+  Cases_on `envty` >>
+  SIMP_TAC std_ss [bir_envty_includes_vs_def, SUBSET_DEF] >>
+  METIS_TAC[]
+);
+
+
+
+
+
+(* ===================== *)
+(*
+bir_vs_consistent!!!
+
+val bir_var_set_is_well_typed_def = Define `bir_var_set_is_well_typed vs <=>
+  (!v1 v2. (v1 IN vs /\ v2 IN vs /\ (bir_var_name v1 = bir_var_name v2)) ==>
+           (bir_var_type v1 = bir_var_type v2))`;
+
+val bir_var_set_is_well_typed_INJ_DEF = store_thm ("bir_var_set_is_well_typed_INJ_DEF",
+  ``bir_var_set_is_well_typed vs <=> INJ bir_var_name vs UNIV``,
+
+SIMP_TAC std_ss [bir_var_set_is_well_typed_def, INJ_DEF, IN_UNIV,
+  bir_var_eq_EXPAND] >>
+METIS_TAC[]);
+
+val bir_var_set_is_well_typed_EMPTY = store_thm ("bir_var_set_is_well_typed_EMPTY",
+  ``bir_var_set_is_well_typed {}``,
+SIMP_TAC std_ss [bir_var_set_is_well_typed_def, NOT_IN_EMPTY]);
+
+val bir_var_set_is_well_typed_INSERT = store_thm ("bir_var_set_is_well_typed_INSERT",
+  ``!v vs. bir_var_set_is_well_typed (v INSERT vs) <=>
+           bir_var_set_is_well_typed vs /\
+           (!v'. v' IN vs ==>
+                 (bir_var_name v = bir_var_name v') ==>
+                 (bir_var_type v = bir_var_type v'))``,
+
+SIMP_TAC std_ss [bir_var_set_is_well_typed_def, IN_INSERT] >>
+METIS_TAC[]);
+
+
+val bir_var_set_is_well_typed_UNION = store_thm ("bir_var_set_is_well_typed_UNION",
+``!vs1 vs2. bir_var_set_is_well_typed (vs1 UNION vs2) <=>
+            bir_var_set_is_well_typed vs1 /\
+            bir_var_set_is_well_typed vs2 /\
+            (!v1 v2. v1 IN vs1 ==> v2 IN vs2 ==>
+                 (bir_var_name v1 = bir_var_name v2) ==>
+                 (bir_var_type v1 = bir_var_type v2))``,
+
+SIMP_TAC std_ss [bir_var_set_is_well_typed_def, IN_UNION] >>
+METIS_TAC[]);
+
+
+val bir_var_set_is_well_typed_SUBSET = store_thm ("bir_var_set_is_well_typed_SUBSET",
+  ``!vs1 vs2. vs1 SUBSET vs2 ==> bir_var_set_is_well_typed vs2 ==> bir_var_set_is_well_typed vs1``,
+SIMP_TAC std_ss [bir_var_set_is_well_typed_def, SUBSET_DEF] >>
+METIS_TAC[]);
+
+
+val bir_env_vars_are_initialised_WELL_TYPED = store_thm ("bir_env_vars_are_initialised_WELL_TYPED",
+  ``!vs env. bir_env_vars_are_initialised env vs ==> bir_var_set_is_well_typed vs``,
+
+  SIMP_TAC std_ss [bir_var_set_is_well_typed_def, bir_env_vars_are_initialised_def] >>
+  REPEAT STRIP_TAC >>
+  Cases_on `v1` >> Cases_on `v2` >>
+  rename1 `bir_var_name (BVar vn1 vty1) = bir_var_name (BVar vn2 vty2)` >>
+  FULL_SIMP_TAC std_ss [bir_var_name_def, bir_var_type_def] >>
+
+
+  `bir_env_var_is_initialised env (BVar vn2 vty1)` by METIS_TAC[] >>
+  `bir_env_var_is_initialised env (BVar vn2 vty2)` by METIS_TAC[] >>
+  FULL_SIMP_TAC std_ss [bir_env_var_is_initialised_def, bir_var_type_def, bir_var_name_def] >>
+  FULL_SIMP_TAC std_ss []
+);
+
+
+val bir_env_vars_are_initialised_SUBSET_DOMAIN = store_thm ("bir_env_vars_are_initialised_SUBSET_DOMAIN",
+  ``!vs env. bir_env_vars_are_initialised env vs ==>
+             (IMAGE bir_var_name vs) SUBSET (bir_env_domain env)``,
+
+REPEAT STRIP_TAC >>
+Cases_on `env` >> rename1 `BEnv env` >>
+FULL_SIMP_TAC std_ss [bir_env_vars_are_initialised_def, SUBSET_DEF, IN_IMAGE,
+  PULL_EXISTS, bir_env_domain_def] >>
+REPEAT STRIP_TAC >>
+rename1 `v IN vs` >>
+Q.PAT_X_ASSUM `!v. _` (MP_TAC o Q.SPEC `v`) >>
+Cases_on `v` >> rename1 `BVar vn vty` >>
+ASM_SIMP_TAC std_ss [bir_env_var_is_initialised_def, bir_env_lookup_def,
+    flookup_thm, PULL_EXISTS, bir_var_name_def]);
+
+
+val VAR_SET_FINITE_IFF_NAME_SET_FINITE = store_thm ("VAR_SET_FINITE_IFF_NAME_SET_FINITE",
+``!vs. FINITE vs <=> FINITE (IMAGE bir_var_name vs)``,
+
+GEN_TAC >> EQ_TAC >- (
+  METIS_TAC[IMAGE_FINITE]
+) >>
+STRIP_TAC >>
+Q.ABBREV_TAC `VS = BIGUNION (IMAGE (\vn. IMAGE (\ty. BVar vn ty) UNIV) (IMAGE bir_var_name vs))` >>
+`vs SUBSET VS` by (
+  Q.UNABBREV_TAC `VS` >>
+  SIMP_TAC std_ss [SUBSET_DEF, IN_BIGUNION, IN_IMAGE, PULL_EXISTS, IN_UNIV] >>
+  REPEAT STRIP_TAC >>
+  rename1 `v IN vs` >>
+  Q.EXISTS_TAC `v` >>
+  Q.EXISTS_TAC `bir_var_type v` >>
+  Cases_on `v` >>
+  ASM_SIMP_TAC std_ss [bir_var_type_def, bir_var_name_def]
+) >>
+
+`FINITE VS` suffices_by METIS_TAC[SUBSET_FINITE] >>
+Q.UNABBREV_TAC `VS` >>
+SIMP_TAC std_ss [FINITE_BIGUNION_EQ, IN_IMAGE, PULL_EXISTS] >>
+METIS_TAC[IMAGE_FINITE, bir_type_t_FINITE_UNIV]);
+
+
+val bir_env_vars_are_initialised_FINITE = store_thm ("bir_env_vars_are_initialised_FINITE",
+  ``!vs env. bir_env_vars_are_initialised env vs ==> FINITE vs``,
+
+METIS_TAC[bir_env_vars_are_initialised_SUBSET_DOMAIN, bir_env_domain_FINITE,
+          VAR_SET_FINITE_IFF_NAME_SET_FINITE, SUBSET_FINITE]);
+
+
+
+val bir_env_vars_are_initialised_ENV_EXISTS_EXTENSION = store_thm ("bir_env_vars_are_initialised_ENV_EXISTS_EXTENSION",
+  ``!vs1 vs2 env1.
+      (FINITE vs2 /\ vs1 SUBSET vs2 /\ bir_var_set_is_well_typed vs2) ==>
+      bir_env_vars_are_initialised env1 vs1 ==>
+      (?env2. bir_env_EQ_FOR_VARS vs1 env1 env2 /\
+              bir_env_vars_are_initialised env2 vs2)``,
+
+REPEAT STRIP_TAC >>
+Cases_on `env1` >> rename1 `BEnv env` >>
+Q.ABBREV_TAC `VF = (\v. (bir_var_type v, SOME (bir_default_value_of_type (bir_var_type v))))` >>
+Q.ABBREV_TAC `M1 = FUN_FMAP VF (vs2 DIFF vs1)` >>
+EXISTS_TAC ``BEnv (FUNION (MAP_KEYS bir_var_name M1) env)`` >>
+
+`FDOM M1 = vs2 DIFF vs1` by METIS_TAC[FDOM_FMAP, FINITE_DIFF] >>
+`INJ bir_var_name (FDOM M1) UNIV` by METIS_TAC [bir_var_set_is_well_typed_INJ_DEF,
+  INJ_SUBSET, SUBSET_REFL, DIFF_SUBSET] >>
+
+`!v v'. v IN vs2 ==> (
+    ((bir_var_name v = bir_var_name v') /\ v' IN (vs2 DIFF vs1)) <=>
+    (~(v IN vs1) /\ (v' = v)))` by (
+
+  SIMP_TAC std_ss [IN_DIFF] >> REPEAT STRIP_TAC >>
+  METIS_TAC[bir_var_set_is_well_typed_def, SUBSET_DEF, bir_var_eq_EXPAND]
+) >>
+
+REPEAT STRIP_TAC >- (
+  SIMP_TAC std_ss [bir_env_EQ_FOR_VARS_def] >>
+  REPEAT STRIP_TAC >>
+  `v IN vs2` by METIS_TAC[SUBSET_DEF] >>
+  ASM_SIMP_TAC std_ss [bir_env_lookup_def, FLOOKUP_FUNION, FLOOKUP_MAP_KEYS]
+) >>
+
+FULL_SIMP_TAC std_ss [bir_env_vars_are_initialised_def]  >>
+Cases >> rename1 `BVar vn vty` >>
+STRIP_TAC >>
+REPEAT (Q.PAT_X_ASSUM `!v. _` (MP_TAC o Q.SPEC `BVar vn vty`)) >>
+FULL_SIMP_TAC std_ss [bir_env_var_is_initialised_def,
+  bir_env_lookup_def, FLOOKUP_MAP_KEYS,
+  FLOOKUP_FUNION, bir_var_name_def] >>
+Cases_on `BVar vn vty IN vs1` >- (
+  ASM_SIMP_TAC std_ss []
+) >>
+Q.UNABBREV_TAC `M1` >>
+Q.UNABBREV_TAC `VF` >>
+ASM_SIMP_TAC std_ss [FLOOKUP_FUN_FMAP, FINITE_DIFF,
+  bir_default_value_of_type_SPEC, bir_var_type_def, IN_DIFF]);
+
+
+
+val bir_env_vars_are_initialised_ENV_EXISTS_IFF = store_thm ("bir_env_vars_are_initialised_ENV_EXISTS_IFF",
+  ``!vs. (?env. bir_env_vars_are_initialised env vs) <=> (FINITE vs /\ bir_var_set_is_well_typed vs)``,
+
+GEN_TAC >> EQ_TAC >- (
+  METIS_TAC[bir_env_vars_are_initialised_WELL_TYPED, bir_env_vars_are_initialised_FINITE]
+) >>
+REPEAT STRIP_TAC >>
+MP_TAC (Q.SPECL [`{}`, `vs`, `bir_empty_env`] bir_env_vars_are_initialised_ENV_EXISTS_EXTENSION) >>
+ASM_SIMP_TAC std_ss [EMPTY_SUBSET, bir_env_vars_are_initialised_EMPTY, NOT_IN_EMPTY,
+  bir_env_EQ_FOR_VARS_EMPTY]);
+
 *)
+
+
+(* ===================== *)
 
 
 (* Equivalence for sets of vars *)
 val bir_env_EQ_FOR_VARS_def = Define `
   bir_env_EQ_FOR_VARS vs env1 env2 <=>
-    (!v.
-      v IN vs ==>
-      (bir_env_lookup (bir_var_name v) env1 =
-        bir_env_lookup (bir_var_name v) env2
-      )
-    )`
+  (!v. v IN vs ==> (bir_env_lookup (bir_var_name v) env1 = bir_env_lookup (bir_var_name v) env2))`
 
-val bir_env_EQ_FOR_VARS_EQUIV_EQ =
-  store_thm ("bir_env_EQ_FOR_VARS_EQUIV_EQ",
-  ``!vs env1 env2.
-      (bir_env_EQ_FOR_VARS vs env1 env2) <=>
-        (bir_env_EQ_FOR_VARS vs env1 =
-          bir_env_EQ_FOR_VARS vs env2
-        )``,
+val bir_env_EQ_FOR_VARS_EQUIV_EQ = store_thm ("bir_env_EQ_FOR_VARS_EQUIV_EQ",
+  ``!vs env1 env2. (bir_env_EQ_FOR_VARS vs env1 env2) <=>
+                   (bir_env_EQ_FOR_VARS vs env1 = bir_env_EQ_FOR_VARS vs env2)``,
 
 SIMP_TAC std_ss [bir_env_EQ_FOR_VARS_def, FUN_EQ_THM] >>
-METIS_TAC []
-);
+METIS_TAC[]);
 
 
-val bir_env_EQ_FOR_VARS_EQUIV =
-  store_thm ("bir_env_EQ_FOR_VARS_EQUIV",
+val bir_env_EQ_FOR_VARS_EQUIV = store_thm ("bir_env_EQ_FOR_VARS_EQUIV",
  ``(!vs env. bir_env_EQ_FOR_VARS vs env env) /\
-   (!vs env1 env2.
-     (bir_env_EQ_FOR_VARS vs env1 env2 <=>
-       (bir_env_EQ_FOR_VARS vs env2 env1)
-     )
-   ) /\
-   (!vs env1 env2 env3.
-     bir_env_EQ_FOR_VARS vs env1 env2 ==>
-     bir_env_EQ_FOR_VARS vs env2 env3 ==>
-     bir_env_EQ_FOR_VARS vs env1 env3
-   )``,
-
-SIMP_TAC std_ss [bir_env_EQ_FOR_VARS_def] >>
-METIS_TAC []
-);
+   (!vs env1 env2. (bir_env_EQ_FOR_VARS vs env1 env2 <=> (bir_env_EQ_FOR_VARS vs env2 env1))) /\
+   (!vs env1 env2 env3. bir_env_EQ_FOR_VARS vs env1 env2 ==>
+                        bir_env_EQ_FOR_VARS vs env2 env3 ==>
+                        bir_env_EQ_FOR_VARS vs env1 env3)``,
+SIMP_TAC std_ss [bir_env_EQ_FOR_VARS_def] >> METIS_TAC[]);
 
 
 
-val bir_env_EQ_FOR_VARS_EMPTY =
-  store_thm ("bir_env_EQ_FOR_VARS_EMPTY",
+val bir_env_EQ_FOR_VARS_EMPTY = store_thm ("bir_env_EQ_FOR_VARS_EMPTY",
   ``!env1 env2. bir_env_EQ_FOR_VARS EMPTY env1 env2``,
-
-SIMP_TAC std_ss [bir_env_EQ_FOR_VARS_def, NOT_IN_EMPTY,
-                 bir_env_EQ_FOR_VARS_def]
-);
+SIMP_TAC std_ss [bir_env_EQ_FOR_VARS_def, NOT_IN_EMPTY, bir_env_EQ_FOR_VARS_def]);
 
 
-val bir_env_EQ_FOR_VARS_UNIV =
-  store_thm ("bir_env_EQ_FOR_VARS_UNIV",
-  ``!env1 env2.
-      bir_env_EQ_FOR_VARS UNIV env1 env2 <=> (env1 = env2)``,
-
+val bir_env_EQ_FOR_VARS_UNIV = store_thm ("bir_env_EQ_FOR_VARS_UNIV",
+  ``!env1 env2. bir_env_EQ_FOR_VARS UNIV env1 env2 <=> (env1 = env2)``,
 REPEAT Cases >>
-SIMP_TAC (std_ss++DatatypeSimps.expand_type_quants_ss[``:bir_var_t``]) [bir_env_EQ_FOR_VARS_def, IN_UNIV,
-    bir_var_environment_t_11, bir_env_lookup_def, bir_var_name_def,
-    FUN_EQ_THM]
-);
+SIMP_TAC (std_ss++DatatypeSimps.expand_type_quants_ss [``:bir_var_t``]) [
+  bir_env_EQ_FOR_VARS_def, IN_UNIV,
+  bir_var_environment_t_11, bir_env_lookup_def, bir_var_name_def, FUN_EQ_THM]);
 
 
-val bir_env_EQ_FOR_VARS_SUBSET =
-  store_thm ("bir_env_EQ_FOR_VARS_SUBSET",
-  ``!vs1 vs2 env1 env2.
-      vs2 SUBSET vs1 ==>
-      bir_env_EQ_FOR_VARS vs1 env1 env2 ==>
-      bir_env_EQ_FOR_VARS vs2 env1 env2``,
-
+val bir_env_EQ_FOR_VARS_SUBSET = store_thm ("bir_env_EQ_FOR_VARS_SUBSET",
+  ``!vs1 vs2 env1 env2. vs2 SUBSET vs1 ==> bir_env_EQ_FOR_VARS vs1 env1 env2 ==> bir_env_EQ_FOR_VARS vs2 env1 env2``,
 SIMP_TAC std_ss [bir_env_EQ_FOR_VARS_def, SUBSET_DEF] >>
-METIS_TAC []
-);
+METIS_TAC[]);
 
 
-val bir_env_EQ_FOR_VARS_read_IMPL =
-  store_thm ("bir_env_EQ_FOR_VARS_read_IMPL",
-  ``!vs env1 env2.
-      bir_env_EQ_FOR_VARS vs env1 env2 ==>
-      (!v.
-        v IN vs ==>
-        (bir_env_read v env1 = bir_env_read v env2)
-      )``,
-
+val bir_env_EQ_FOR_VARS_read_IMPL = store_thm ("bir_env_EQ_FOR_VARS_read_IMPL",
+``!vs env1 env2. bir_env_EQ_FOR_VARS vs env1 env2 ==>
+  (!v. v IN vs ==> (bir_env_read v env1 = bir_env_read v env2))``,
 SIMP_TAC std_ss [bir_env_EQ_FOR_VARS_def] >>
-METIS_TAC [bir_env_read_EQ_lookup_IMPL]
-);
+METIS_TAC[bir_env_read_EQ_lookup_IMPL]);
 
 
 val _ = export_theory();
