src/theory/bir/bir_expScript.sml
@@ -16,9 +16,7 @@ val bir_type_ss = rewrites ((type_rws ``:bir_type_t``));
 
 val _ = Datatype `bir_exp_t =
     BExp_Const             bir_imm_t
-  | BExp_MemConst          bir_immtype_t (* Address type *)
-                           bir_immtype_t (* Value type *)
-                           (num |-> num) (* Memory map *)
+  | BExp_MemConst          bir_immtype_t (*Addr-Type*) bir_immtype_t (* value-type *) (num |-> num)
   | BExp_Den               bir_var_t
 
   | BExp_Cast              bir_cast_t bir_exp_t bir_immtype_t
@@ -41,124 +39,89 @@ val _ = Datatype `bir_exp_t =
 (* ------------------------------------------------------------------------- *)
 
 val bir_eval_cast_def = Define `
-  (bir_eval_cast ct (BVal_Known (BKVal_Imm bi)) ty =
-    (BVal_Known (BKVal_Imm (bir_gencast ct bi ty)))
-  ) /\
-  (bir_eval_cast _ _ _ = BVal_Unknown)`;
+  (bir_eval_cast ct (SOME (BVal_Imm bi)) ty = SOME (BVal_Imm (bir_gencast ct bi ty))) /\
+  (bir_eval_cast _ _ _ = NONE)`;
 
 val bir_eval_unary_exp_def = Define `
-  (bir_eval_unary_exp et (BVal_Known (BKVal_Imm bi)) =
-    (BVal_Known (BKVal_Imm (bir_unary_exp et bi)))
-  ) /\
-  (bir_eval_unary_exp _ _ = BVal_Unknown)`;
+  (bir_eval_unary_exp et (SOME (BVal_Imm bi)) = SOME (BVal_Imm (bir_unary_exp et bi))) /\
+  (bir_eval_unary_exp _ _ = NONE)`;
 
 val bir_eval_bin_exp_def = Define `
-  (bir_eval_bin_exp et (BVal_Known (BKVal_Imm bi1))
-                       (BVal_Known (BKVal_Imm bi2)) =
-     if (type_of_bir_imm bi1 <> type_of_bir_imm bi2)
-     then BVal_Unknown
-     else (BVal_Known (BKVal_Imm (bir_bin_exp et bi1 bi2)))
-  ) /\
-  (bir_eval_bin_exp _ _ _ = BVal_Unknown)`;
+  (bir_eval_bin_exp et (SOME (BVal_Imm bi1)) (SOME (BVal_Imm bi2)) =
+     if (type_of_bir_imm bi1 <> type_of_bir_imm bi2) then NONE else
+     SOME (BVal_Imm (bir_bin_exp et bi1 bi2))) /\
+  (bir_eval_bin_exp _ _ _ = NONE)`;
 
 val bir_eval_bin_pred_def = Define `
-  (bir_eval_bin_pred pt (BVal_Known (BKVal_Imm bi1))
-                        (BVal_Known (BKVal_Imm bi2)) =
-     if (type_of_bir_imm bi1 <> type_of_bir_imm bi2)
-     then BVal_Unknown
-     else BVal_Known (BKVal_Imm (bool2b (bir_bin_pred pt bi1 bi2)))
-  ) /\
-  (bir_eval_bin_pred _ _ _ = BVal_Unknown)`;
+  (bir_eval_bin_pred pt (SOME (BVal_Imm bi1)) (SOME (BVal_Imm bi2)) =
+     if (type_of_bir_imm bi1 <> type_of_bir_imm bi2) then NONE else
+     SOME (BVal_Imm (bool2b (bir_bin_pred pt bi1 bi2)))) /\
+  (bir_eval_bin_pred _ _ _ = NONE)`;
 
 val bir_eval_memeq_def = Define `
-  (bir_eval_memeq (BVal_Known (BKVal_Mem at1 vt1 mmap1))
-                  (BVal_Known (BKVal_Mem at2 vt2 mmap2)) =
-     if ((at1 <> at2) \/ (vt1 <> vt2))
-     then BVal_Unknown
-     else BVal_Known (BKVal_Imm (bool2b
-            (bir_memeq at1 vt1 mmap1 mmap2))
-          )
-  ) /\
-  (bir_eval_memeq _ _ = BVal_Unknown)`;
+  (bir_eval_memeq (SOME (BVal_Mem at1 vt1 mmap1)) (SOME (BVal_Mem at2 vt2 mmap2)) =
+     if ((at1 <> at2) \/ (vt1 <> vt2)) then NONE else
+     SOME(BVal_Imm (bool2b (bir_memeq at1 vt1 mmap1 mmap2)))) /\
+  (bir_eval_memeq _ _ = NONE)`;
 
 val bir_eval_ifthenelse_def = Define `
-  (bir_eval_ifthenelse (BVal_Known (BKVal_Imm (Imm1 cw))) v1 v2 =
-     if (type_of_bir_val v1 <> type_of_bir_val v2)
-     then BVal_Unknown
-     else
-       if (cw = 1w) then v1 else v2
-  ) /\
-  (bir_eval_ifthenelse _ _ _ = BVal_Unknown)`;
+  (bir_eval_ifthenelse (SOME (BVal_Imm (Imm1 cw))) (SOME v1) (SOME v2) =
+     if (type_of_bir_val v1 <> type_of_bir_val v2) then NONE else
+       if (cw = 1w) then SOME v1 else SOME v2) /\
+  (bir_eval_ifthenelse _ _ _ = NONE)`;
 
 val bir_eval_load_def = Define `
-  (bir_eval_load (BVal_Known (BKVal_Mem ta tv mmap))
-                 (BVal_Known (BKVal_Imm a)) en t =
-     if ((type_of_bir_imm a) = ta)
-     then (case (bir_load_from_mem tv t ta mmap en (b2n a)) of
-             NONE => BVal_Unknown
-           | SOME i => BVal_Known (BKVal_Imm i)
-          )
-     else BVal_Unknown
-  ) /\
-  (bir_eval_load _ _ _ _ = BVal_Unknown)`;
+  (bir_eval_load (SOME (BVal_Mem ta tv mmap)) (SOME (BVal_Imm a)) en t =
+     if ((type_of_bir_imm a) = ta) then
+        (case (bir_load_from_mem tv t ta mmap en (b2n a)) of
+           NONE => NONE
+         | SOME i => SOME (BVal_Imm i))
+     else NONE) /\
+  (bir_eval_load _ _ _ _ = NONE)`;
 
 val bir_eval_store_def = Define `
-  (bir_eval_store (BVal_Known (BKVal_Mem ta tv mmap))
-                  (BVal_Known (BKVal_Imm a)) en
-                  (BVal_Known (BKVal_Imm v)) =
+  (bir_eval_store (SOME (BVal_Mem ta tv mmap)) (SOME (BVal_Imm a)) en (SOME (BVal_Imm v)) =
      if ((type_of_bir_imm a) = ta) then
         (case (bir_store_in_mem tv ta v mmap en (b2n a)) of
-           NONE => BVal_Unknown
-         | SOME mmap' => BVal_Known (BKVal_Mem ta tv mmap'))
-     else BVal_Unknown) /\
-  (bir_eval_store _ _ _ _ = BVal_Unknown)`;
+           NONE => NONE
+         | SOME mmap' => SOME (BVal_Mem ta tv mmap'))
+     else NONE) /\
+  (bir_eval_store _ _ _ _ = NONE)`;
+
 
 
 val bir_eval_exp_def = Define `
-  (bir_eval_exp (BExp_Const n) env = BVal_Known (BKVal_Imm n)) /\
+  (bir_eval_exp (BExp_Const n) env = SOME (BVal_Imm n)) /\
 
-  (bir_eval_exp (BExp_MemConst aty vty mmap) env =
-    BVal_Known (BKVal_Mem aty vty mmap)
-  ) /\
+  (bir_eval_exp (BExp_MemConst aty vty mmap) env = SOME (BVal_Mem aty vty mmap)) /\
 
   (bir_eval_exp (BExp_Den v) env = bir_env_read v env) /\
 
-  (bir_eval_exp (BExp_Cast ct e ty) env = 
-    bir_eval_cast ct (bir_eval_exp e env) ty
-  ) /\
+  (bir_eval_exp (BExp_Cast ct e ty) env = (
+     bir_eval_cast ct (bir_eval_exp e env) ty)) /\
 
-  (bir_eval_exp (BExp_UnaryExp et e) env = 
-    bir_eval_unary_exp et (bir_eval_exp e env)
-  ) /\
+  (bir_eval_exp (BExp_UnaryExp et e) env = (
+     bir_eval_unary_exp et (bir_eval_exp e env))) /\
 
-  (bir_eval_exp (BExp_BinExp et e1 e2) env = 
-    bir_eval_bin_exp et (bir_eval_exp e1 env)
-                        (bir_eval_exp e2 env)
-  ) /\
+  (bir_eval_exp (BExp_BinExp et e1 e2) env = (
+     bir_eval_bin_exp et (bir_eval_exp e1 env) (bir_eval_exp e2 env))) /\
 
-  (bir_eval_exp (BExp_BinPred pt e1 e2) env =
-    bir_eval_bin_pred pt (bir_eval_exp e1 env)
-                         (bir_eval_exp e2 env)
-  ) /\
+  (bir_eval_exp (BExp_BinPred pt e1 e2) env = (
+     bir_eval_bin_pred pt (bir_eval_exp e1 env) (bir_eval_exp e2 env))) /\
 
-  (bir_eval_exp (BExp_MemEq e1 e2) env =
-    bir_eval_memeq (bir_eval_exp e1 env) (bir_eval_exp e2 env)
-  ) /\
+  (bir_eval_exp (BExp_MemEq e1 e2) env = (
+     bir_eval_memeq (bir_eval_exp e1 env) (bir_eval_exp e2 env))) /\
+
 
   (bir_eval_exp (BExp_IfThenElse c et ef) env =
-    bir_eval_ifthenelse (bir_eval_exp c env) (bir_eval_exp et env)
-                        (bir_eval_exp ef env)
+     bir_eval_ifthenelse (bir_eval_exp c env) (bir_eval_exp et env) (bir_eval_exp ef env)
   ) /\
 
   (bir_eval_exp (BExp_Load mem_e a_e en ty) env =
-    bir_eval_load (bir_eval_exp mem_e env) (bir_eval_exp a_e env)
-                   en ty
-  ) /\
+     bir_eval_load (bir_eval_exp mem_e env) (bir_eval_exp a_e env) en ty) /\
 
   (bir_eval_exp (BExp_Store mem_e a_e en v_e) env =
-    bir_eval_store (bir_eval_exp mem_e env) (bir_eval_exp a_e env)
-                   en (bir_eval_exp v_e env)
-  )
+     bir_eval_store (bir_eval_exp mem_e env) (bir_eval_exp a_e env) en (bir_eval_exp v_e env))
 `;
 
 
@@ -169,645 +132,343 @@ val bir_eval_exp_def = Define `
 (* ------------------------------------------------------------------------- *)
 
 val bir_eval_cast_REWRS = store_thm ("bir_eval_cast_REWRS",
-  ``(!ct bi ty.
-      (bir_eval_cast ct (BVal_Known (BKVal_Imm bi)) ty =
-        BVal_Known (BKVal_Imm (bir_gencast ct bi ty))
-      )
-    ) /\
-    (!ct ty. bir_eval_cast ct BVal_Unknown ty = BVal_Unknown) /\
-    (!ct at vt mmap ty.
-      bir_eval_cast ct (BVal_Known (BKVal_Mem at vt mmap)) ty =
-        BVal_Unknown
-    )``,
+``(!ct bi ty. (bir_eval_cast ct (SOME (BVal_Imm bi)) ty = SOME (BVal_Imm (bir_gencast ct bi ty)))) /\
+  (!ct ty. bir_eval_cast ct NONE ty = NONE) /\
+  (!ct at vt mmap ty. bir_eval_cast ct (SOME (BVal_Mem at vt mmap)) ty = NONE)``,
+SIMP_TAC std_ss [bir_eval_cast_def]);
 
-SIMP_TAC std_ss [bir_eval_cast_def]
-);
-
-val bir_eval_unary_exp_REWRS =
-  store_thm ("bir_eval_unary_exp_REWRS",
-  ``(!et bi.
-      (bir_eval_unary_exp et (BVal_Known (BKVal_Imm bi)) =
-        BVal_Known (BKVal_Imm (bir_unary_exp et bi))
-      )
-    ) /\
-    (!et. bir_eval_unary_exp et BVal_Unknown = BVal_Unknown) /\
-    (!et at vt mmap.
-      bir_eval_unary_exp et (BVal_Known (BKVal_Mem at vt mmap)) =
-        BVal_Unknown
-    )``,
-
+val bir_eval_unary_exp_REWRS = store_thm ("bir_eval_unary_exp_REWRS",
+ ``(!et bi. (bir_eval_unary_exp et (SOME (BVal_Imm bi)) = SOME (BVal_Imm (bir_unary_exp et bi)))) /\
+   (!et. bir_eval_unary_exp et NONE = NONE) /\
+   (!et at vt mmap. bir_eval_unary_exp et (SOME (BVal_Mem at vt mmap)) = NONE)``,
 SIMP_TAC std_ss [bir_eval_unary_exp_def]);
 
 
 val bir_eval_bin_exp_REWRS = store_thm ("bir_eval_bin_exp_REWRS",
-``(!et bi1 bi2.
-    bir_eval_bin_exp et (BVal_Known (BKVal_Imm bi1))
-                        (BVal_Known (BKVal_Imm bi2)) =
-      if (type_of_bir_imm bi1 <> type_of_bir_imm bi2)
-      then BVal_Unknown
-      else BVal_Known (BKVal_Imm (bir_bin_exp et bi1 bi2))
-  ) /\
-  (!et v. bir_eval_bin_exp et BVal_Unknown v = BVal_Unknown) /\
-  (!et v. bir_eval_bin_exp et v BVal_Unknown = BVal_Unknown) /\
-  (!et at vt mmap v.
-    bir_eval_bin_exp et (BVal_Known (BKVal_Mem at vt mmap)) v =
-      BVal_Unknown
-  ) /\
-  (!et at vt mmap v.
-    bir_eval_bin_exp et v (BVal_Known (BKVal_Mem at vt mmap)) =
-      BVal_Unknown
-  )``,
-
+``(!et bi1 bi2. bir_eval_bin_exp et (SOME (BVal_Imm bi1)) (SOME (BVal_Imm bi2)) =
+     if (type_of_bir_imm bi1 <> type_of_bir_imm bi2) then NONE else
+     SOME (BVal_Imm (bir_bin_exp et bi1 bi2))) /\
+  (!et v. bir_eval_bin_exp et NONE v = NONE) /\
+  (!et v. bir_eval_bin_exp et v NONE = NONE) /\
+  (!et at vt mmap v. bir_eval_bin_exp et (SOME (BVal_Mem at vt mmap)) v = NONE) /\
+  (!et at vt mmap v. bir_eval_bin_exp et v (SOME (BVal_Mem at vt mmap)) = NONE)``,
 SIMP_TAC std_ss [bir_eval_bin_exp_def] >>
 CONJ_TAC >> (
-  Cases_on `v` >| [
-    SIMP_TAC std_ss [bir_eval_bin_exp_def],
-
-    Cases_on `b` >> SIMP_TAC std_ss [bir_eval_bin_exp_def]
-  ]
-)
-);
+  Cases_on `v` >> (TRY (Q.SPEC_TAC (`x`, `k`) >> Cases_on `k`)) >>
+    (SIMP_TAC std_ss [bir_eval_bin_exp_def])
+));
 
 val bir_eval_bin_pred_REWRS = store_thm ("bir_eval_bin_pred_REWRS",
-  ``(!et bi1 bi2.
-      bir_eval_bin_pred et (BVal_Known (BKVal_Imm bi1))
-                           (BVal_Known (BKVal_Imm bi2)) =
-      if (type_of_bir_imm bi1 <> type_of_bir_imm bi2)
-      then BVal_Unknown
-      else
-        BVal_Known (BKVal_Imm (bool2b (bir_bin_pred et bi1 bi2)))
-    ) /\
-    (!et v. bir_eval_bin_pred et BVal_Unknown v = BVal_Unknown) /\
-    (!et v. bir_eval_bin_pred et v BVal_Unknown = BVal_Unknown) /\
-    (!et at vt mmap v.
-      bir_eval_bin_pred et (BVal_Known (BKVal_Mem at vt mmap)) v =
-        BVal_Unknown
-    ) /\
-    (!et at vt mmap v.
-      bir_eval_bin_pred et v (BVal_Known (BKVal_Mem at vt mmap)) =
-        BVal_Unknown
-    )``,
-
+``(!et bi1 bi2. bir_eval_bin_pred et (SOME (BVal_Imm bi1)) (SOME (BVal_Imm bi2)) =
+     if (type_of_bir_imm bi1 <> type_of_bir_imm bi2) then NONE else
+     SOME (BVal_Imm (bool2b (bir_bin_pred et bi1 bi2)))) /\
+  (!et v. bir_eval_bin_pred et NONE v = NONE) /\
+  (!et v. bir_eval_bin_pred et v NONE = NONE) /\
+  (!et at vt mmap v. bir_eval_bin_pred et (SOME (BVal_Mem at vt mmap)) v = NONE) /\
+  (!et at vt mmap v. bir_eval_bin_pred et v (SOME (BVal_Mem at vt mmap)) = NONE)``,
 SIMP_TAC std_ss [bir_eval_bin_pred_def] >>
 CONJ_TAC >> (
-  Cases_on `v` >| [
-    SIMP_TAC std_ss [bir_eval_bin_pred_def],
-
-    Cases_on `b` >> SIMP_TAC std_ss [bir_eval_bin_pred_def]
-  ]
-)
-);
+  Cases_on `v` >> (TRY (Q.SPEC_TAC (`x`, `k`) >> Cases_on `k`)) >>
+    (SIMP_TAC std_ss [bir_eval_bin_pred_def])
+));
 
 val bir_eval_memeq_REWRS = store_thm ("bir_eval_memeq_REWRS",
-  ``(!at1 vt1 mmap1 at2 vt2 mmap2.
-      (bir_eval_memeq (BVal_Known (BKVal_Mem at1 vt1 mmap1))
-                      (BVal_Known (BKVal_Mem at2 vt2 mmap2)) =
-        if ((at1 <> at2) \/ (vt1 <> vt2))
-        then BVal_Unknown
-        else BVal_Known (BKVal_Imm
-               (bool2b (bir_memeq at1 vt1 mmap1 mmap2))
-             )
-      )
-    ) /\
-    (!v. bir_eval_memeq BVal_Unknown v = BVal_Unknown) /\
-    (!v. bir_eval_memeq v BVal_Unknown = BVal_Unknown) /\
-    (!bi v.
-      bir_eval_memeq (BVal_Known (BKVal_Imm bi)) v =
-        BVal_Unknown
-    ) /\
-    (!bi v.
-      bir_eval_memeq v (BVal_Known (BKVal_Imm bi)) = BVal_Unknown
-    )``,
-
+ ``(!at1 vt1 mmap1 at2 vt2 mmap2. (bir_eval_memeq (SOME (BVal_Mem at1 vt1 mmap1)) (SOME (BVal_Mem at2 vt2 mmap2)) =
+     if ((at1 <> at2) \/ (vt1 <> vt2)) then NONE else
+     SOME (BVal_Imm (bool2b (bir_memeq at1 vt1 mmap1 mmap2))))) /\
+   (!v. bir_eval_memeq NONE v = NONE) /\
+   (!v. bir_eval_memeq v NONE = NONE) /\
+   (!bi v. bir_eval_memeq (SOME (BVal_Imm bi)) v = NONE) /\
+   (!bi v. bir_eval_memeq v (SOME (BVal_Imm bi)) = NONE)``,
 SIMP_TAC std_ss [bir_eval_memeq_def] >>
 CONJ_TAC >> (
-  Cases_on `v` >| [
-    SIMP_TAC std_ss [bir_eval_memeq_def],
+  Cases_on `v` >> (TRY (Q.SPEC_TAC (`x`, `k`) >> Cases_on `k`)) >>
+    (SIMP_TAC std_ss [bir_eval_memeq_def])
+));
 
-    Cases_on `b` >> SIMP_TAC std_ss [bir_eval_memeq_def]
-  ]
-)
-);
-
-
-val bir_eval_ifthenelse_REWRS =
-  store_thm ("bir_eval_ifthenelse_REWRS",
-  ``(!c v1 v2.
-      bir_eval_ifthenelse (BVal_Known (BKVal_Imm c)) v1 v2 =
-        if (type_of_bir_imm c = Bit1)
-        then (
-	  if (type_of_bir_val v1 <> type_of_bir_val v2)
-          then BVal_Unknown
-          else if (c = Imm1 1w) then v1 else v2
-        )
-        else BVal_Unknown
-    ) /\
-    (!c e1 e2.
-      bir_eval_ifthenelse BVal_Unknown e1 e2 = BVal_Unknown
-    ) /\
-    (!at vt mmap e1 e2.
-      bir_eval_ifthenelse (BVal_Known (BKVal_Mem at vt mmap))
-                          e1 e2 = BVal_Unknown
-    )``,
+val bir_eval_ifthenelse_REWRS = store_thm ("bir_eval_ifthenelse_REWRS",
+``(!c v1 v2. bir_eval_ifthenelse (SOME (BVal_Imm c)) (SOME v1) (SOME v2) =
+     if (type_of_bir_imm c = Bit1) then (
+       if (type_of_bir_val v1 <> type_of_bir_val v2) then NONE else
+         if (c = Imm1 1w) then (SOME v1) else (SOME v2)
+     ) else NONE) /\
+  (!c v2. bir_eval_ifthenelse c NONE v2 = NONE) /\
+  (!c v1. bir_eval_ifthenelse c v1 NONE = NONE) /\
+  (!c e1 e2. bir_eval_ifthenelse NONE e1 e2 = NONE) /\
+  (!at vt mmap e1 e2. bir_eval_ifthenelse (SOME (BVal_Mem at vt mmap)) e1 e2 = NONE)``,
 
 SIMP_TAC std_ss [bir_eval_ifthenelse_def] >>
-Cases_on `c` >> (
-  SIMP_TAC (std_ss++bir_imm_ss) [type_of_bir_imm_def,
-                                 bir_eval_ifthenelse_def]
-)
-);
+REPEAT (CONJ_TAC) >> (
+  Cases_on `c` >>
+  (TRY (Cases_on `x` >>  Cases_on `b` >> TRY (Cases_on `v1`))) >>
+  SIMP_TAC (std_ss++bir_imm_ss) [type_of_bir_imm_def, bir_eval_ifthenelse_def]
+));
 
-val bir_eval_ifthenelse_REWRS_Unknown =
-  store_thm ("bir_eval_ifthenelse_REWRS_Unknown",
-  ``(!vc v1 v2.
-       (type_of_bir_val vc <> SOME (BType_Imm Bit1)) ==>
-       (bir_eval_ifthenelse vc v1 v2 = BVal_Unknown)) /\
-    (!vc v1 v2.
-       ~(bir_val_is_Bool vc) ==>
-       (bir_eval_ifthenelse vc v1 v2 = BVal_Unknown)) /\
-    (!vc v1 v2.
-       (type_of_bir_val v1 <> type_of_bir_val v2) ==>
-       (bir_eval_ifthenelse vc v1 v2 = BVal_Unknown))``,
+val bir_eval_ifthenelse_REWRS_NONE = store_thm ("bir_eval_ifthenelse_REWRS_NONE",
+``(!vc v1 v2.
+     (type_of_bir_val vc <> BType_Imm Bit1) ==>
+     (bir_eval_ifthenelse (SOME vc) v1 v2 = NONE)) /\
+  (!vc v1 v2.
+     ~(bir_val_is_Bool vc) ==>
+     (bir_eval_ifthenelse (SOME vc) v1 v2 = NONE)) /\
+  (!vc v1 v2.
+     (type_of_bir_val v1 <> type_of_bir_val v2) ==>
+     (bir_eval_ifthenelse vc (SOME v1) (SOME v2) = NONE))``,
 
-REPEAT STRIP_TAC >> (
-  Cases_on `vc` >| [
-    FULL_SIMP_TAC (std_ss++bir_type_ss++bir_imm_ss)
-		  [type_of_bir_imm_def, type_of_bir_val_def,
-		   bir_eval_ifthenelse_REWRS,
-                   bir_val_checker_REWRS],
+REPEAT STRIP_TAC >> Cases_on `vc` >> Cases_on `v1` >>  Cases_on `v2` >> (
+  TRY (Cases_on `x`) >>
+  FULL_SIMP_TAC (std_ss++bir_type_ss++bir_imm_ss++optionSimps.OPTION_ss) [type_of_bir_imm_def, type_of_bir_val_def,
+    bir_eval_ifthenelse_REWRS, bir_val_checker_REWRS]
+));
 
-    Cases_on `b` >> (
-      FULL_SIMP_TAC (std_ss++bir_type_ss++bir_imm_ss)
-		    [type_of_bir_imm_def, type_of_bir_val_def,
-		     type_of_bir_kval_def,
-		     bir_eval_ifthenelse_REWRS,
-		     bir_val_checker_REWRS]
-    )
-  ]
-)
-);
-
-val bir_eval_ifthenelse_TF_EQ =
-  store_thm ("bir_eval_ifthenelse_TF_EQ",
-  ``!c v.
-      bir_eval_ifthenelse c v v =
-        if (bir_val_is_Bool c) then v else BVal_Unknown``,
-
-Cases_on `c` >| [
-  SIMP_TAC (std_ss++bir_imm_ss++bir_type_ss)
-           [type_of_bir_imm_def, bir_eval_ifthenelse_REWRS,
-            bir_val_checker_REWRS],
-
-  Cases_on `b` >> (
-    SIMP_TAC (std_ss++bir_imm_ss++bir_type_ss)
-	     [type_of_bir_imm_def, bir_eval_ifthenelse_REWRS,
-	      bir_val_checker_REWRS]
-  )
-]
-);
+val bir_eval_ifthenelse_TF_EQ = store_thm ("bir_eval_ifthenelse_TF_EQ",
+``!c v.
+     bir_eval_ifthenelse (SOME c) v v =
+     if (bir_val_is_Bool c) then v else NONE``,
+Cases_on `c` >> Cases_on `b` >> Cases_on `v` >> (
+  SIMP_TAC (std_ss++bir_imm_ss++bir_type_ss) [type_of_bir_imm_def, bir_eval_ifthenelse_REWRS,
+    bir_val_checker_REWRS]
+));
 
 
-val bir_eval_load_Unknown_REWRS1 = prove (
-  ``(!mem en t.
-      bir_eval_load mem BVal_Unknown en t = BVal_Unknown) /\
-    (!mem en t aty vty mmap.
-      bir_eval_load mem (BVal_Known (BKVal_Mem aty vty mmap)) en t =
-         BVal_Unknown
-    )``,
+val bir_eval_load_NONE_REWRS1 = prove (
+  ``(!mem en t. bir_eval_load mem NONE en t = NONE) /\
+    (!mem en t aty vty mmap. bir_eval_load mem (SOME (BVal_Mem aty vty mmap)) en t = NONE)``,
 
 SIMP_TAC std_ss [bir_eval_load_def] >>
-REPEAT CONJ_TAC >> (
-  Cases_on `mem` >| [
-    SIMP_TAC std_ss [bir_eval_load_def],
+REPEAT CONJ_TAC >>
+Cases_on `mem` >> (TRY (Cases_on `x`)) >> SIMP_TAC std_ss [bir_eval_load_def]);
 
-    Cases_on `b` >> (
-      SIMP_TAC std_ss [bir_eval_load_def]
-    )
-  ]
-)
-);
+val bir_eval_load_NONE_REWRS2 = prove (
+  ``(!a en t. bir_eval_load NONE a en t = NONE) /\
+    (!a en t i. bir_eval_load (SOME (BVal_Imm i)) a en t = NONE)``,
 
-val bir_eval_load_Unknown_REWRS2 = prove (
-  ``(!a en t. bir_eval_load BVal_Unknown a en t = BVal_Unknown) /\
-    (!a en t i.
-      bir_eval_load (BVal_Known (BKVal_Imm i)) a en t =
-        BVal_Unknown
-    )``,
+SIMP_TAC std_ss [bir_eval_load_def]);
 
-SIMP_TAC std_ss [bir_eval_load_def]
-);
-
-val bir_eval_load_Unknown_REWRS3 = prove (
+val bir_eval_load_NONE_REWRS3 = prove (
   ``!a en t i aty vty mmap.
       (type_of_bir_imm i <> aty) ==>
-      (bir_eval_load (BVal_Known (BKVal_Mem aty vty mmap))
-                     (BVal_Known (BKVal_Imm i)) en t = BVal_Unknown
-      )``,
+      (bir_eval_load (SOME (BVal_Mem aty vty mmap)) (SOME (BVal_Imm i)) en t = NONE)``,
 
-SIMP_TAC std_ss [bir_eval_load_def]
-);
+SIMP_TAC std_ss [bir_eval_load_def]);
 
 
-val bir_eval_load_Unknown_REWRS4 = prove (
+val bir_eval_load_NONE_REWRS4 = prove (
   ``!a en t i aty vty mmap.
       (t <> vty) ==>
-      (bir_eval_load (BVal_Known (BKVal_Mem aty vty mmap))
-                     (BVal_Known (BKVal_Imm i)) BEnd_NoEndian t =
-        BVal_Unknown
-      )``,
+      (bir_eval_load (SOME (BVal_Mem aty vty mmap)) (SOME (BVal_Imm i)) BEnd_NoEndian t = NONE)``,
 
 SIMP_TAC std_ss [bir_eval_load_def] >>
 REPEAT STRIP_TAC >>
-COND_CASES_TAC >> (
-  SIMP_TAC std_ss [] >>
-  ASM_SIMP_TAC std_ss [bir_load_from_mem_NO_ENDIAN]
-)
-);
+Cases_on `t` >> Cases_on `vty` >> SIMP_TAC std_ss [] >>
+ASM_SIMP_TAC std_ss [bir_load_from_mem_NO_ENDIAN]);
 
-val bir_eval_load_Unknown_REWRS5 = prove (
+val bir_eval_load_NONE_REWRS5 = prove (
   ``!a en t i aty vty mmap en.
       (bir_number_of_mem_splits vty t aty = NONE) ==>
-      (bir_eval_load (BVal_Known (BKVal_Mem aty vty mmap))
-                     (BVal_Known (BKVal_Imm i)) en t = BVal_Unknown
-      )``,
+      (bir_eval_load (SOME (BVal_Mem aty vty mmap)) (SOME (BVal_Imm i)) en t = NONE)``,
 
 SIMP_TAC std_ss [bir_eval_load_def] >>
 REPEAT STRIP_TAC >>
-COND_CASES_TAC >> (
-  SIMP_TAC std_ss [] >>
-  ASM_SIMP_TAC std_ss [bir_load_from_mem_def]
-)
-);
+Cases_on `t` >> Cases_on `vty` >> SIMP_TAC std_ss [] >>
+ASM_SIMP_TAC std_ss [bir_load_from_mem_def]);
 
 
-val bir_eval_load_Unknown_REWRS =
-  save_thm ("bir_eval_load_Unknown_REWRS",
-
-REWRITE_RULE [GSYM CONJ_ASSOC] (
-  LIST_CONJ [bir_eval_load_Unknown_REWRS1,
-             bir_eval_load_Unknown_REWRS2,
-	     bir_eval_load_Unknown_REWRS3,
-             bir_eval_load_Unknown_REWRS4,
-	     bir_eval_load_Unknown_REWRS5]
-)
-);
+val bir_eval_load_NONE_REWRS = save_thm ("bir_eval_load_NONE_REWRS",
+  REWRITE_RULE [GSYM CONJ_ASSOC] (
+  LIST_CONJ [bir_eval_load_NONE_REWRS1, bir_eval_load_NONE_REWRS2,
+             bir_eval_load_NONE_REWRS3, bir_eval_load_NONE_REWRS4,
+             bir_eval_load_NONE_REWRS5]));
 
 
-val bir_eval_load_SINGLE_REWR =
-  store_thm ("bir_eval_load_SINGLE_REWR",
-  ``!i aty vty mmap en.
-      bir_eval_load (BVal_Known (BKVal_Mem aty vty mmap))
-                    (BVal_Known (BKVal_Imm i)) en vty =
-        if (type_of_bir_imm i = aty)
-        then BVal_Known
-               (BKVal_Imm (n2bs (bir_load_mmap mmap (b2n i)) vty))
-        else BVal_Unknown
-        ``,
+val bir_eval_load_SINGLE_REWR = store_thm ("bir_eval_load_SINGLE_REWR",
+  ``!a en t i aty vty mmap en.
+      (bir_eval_load (SOME (BVal_Mem aty vty mmap)) (SOME (BVal_Imm i)) en vty) =
+      ((if (type_of_bir_imm i = aty) then (SOME (BVal_Imm (n2bs (bir_load_mmap mmap (b2n i)) vty)))
+       else NONE))``,
 
 SIMP_TAC arith_ss [bir_eval_load_def, bir_load_from_mem_SINGLE] >>
 REPEAT STRIP_TAC >>
-COND_CASES_TAC >> ASM_REWRITE_TAC [] >>
+COND_CASES_TAC >> ASM_REWRITE_TAC[] >>
 `bir_mem_addr aty (b2n i) = b2n i` suffices_by ASM_SIMP_TAC std_ss [] >>
 MATCH_MP_TAC bir_mem_addr_id >>
-METIS_TAC [b2n_lt]
+METIS_TAC[b2n_lt]
 );
 
 
-val bir_eval_load_BASIC_REWR =
-  store_thm ("bir_eval_load_BASIC_REWR",
+val bir_eval_load_BASIC_REWR = store_thm ("bir_eval_load_BASIC_REWR",
   ``!a en t i aty vty ty mmap en.
-      bir_eval_load (BVal_Known (BKVal_Mem aty vty mmap))
-                    (BVal_Known (BKVal_Imm i)) en ty =
-        if type_of_bir_imm i = aty
-        then case bir_load_from_mem vty ty aty mmap en (b2n i) of
-               NONE => BVal_Unknown
-             | SOME i => BVal_Known (BKVal_Imm i)
-        else BVal_Unknown``,
-
-SIMP_TAC arith_ss [bir_eval_load_def]
-);
+      (bir_eval_load (SOME (BVal_Mem aty vty mmap)) (SOME (BVal_Imm i)) en ty) =
+      (if type_of_bir_imm i = aty then
+        case bir_load_from_mem vty ty aty mmap en (b2n i) of
+          NONE => NONE
+        | SOME i => SOME (BVal_Imm i)
+       else NONE)``,
+SIMP_TAC arith_ss [bir_eval_load_def]);
 
 
 val bir_eval_load_FULL_REWRS = save_thm ("bir_eval_load_FULL_REWRS",
 let
-  val thm_prune0 = prove (
-    ``(!ta a.
-        (type_of_bir_imm a <> ta) ==>
-        (bir_eval_load (BVal_Known (BKVal_Mem ta tv mmap))
-                       (BVal_Known (BKVal_Imm a)) en tr =
-          BVal_Unknown
-        )
-      ) /\
+  val thm_prune0 = prove (``(!ta a.
+      (type_of_bir_imm a <> ta) ==>
+      (bir_eval_load (SOME (BVal_Mem ta tv mmap)) (SOME (BVal_Imm a)) en tr = NONE)) /\
       (!tr tv.
-        (tr <> tv) ==>
-        (bir_number_of_mem_splits tv tr ta <> NONE) ==>
-        (bir_eval_load (BVal_Known (BKVal_Mem ta tv mmap))
-                       (BVal_Known (BKVal_Imm i)) BEnd_NoEndian tr =
-          BVal_Unknown
-        )
-      ) /\
+      (tr <> tv) ==> (bir_number_of_mem_splits tv tr ta <> NONE) ==>
+      (bir_eval_load (SOME (BVal_Mem ta tv mmap)) (SOME (BVal_Imm i)) BEnd_NoEndian tr = NONE)) /\
       (!tr tv.
-        (bir_number_of_mem_splits tv tr ta = NONE) ==>
-        (bir_eval_load (BVal_Known (BKVal_Mem ta tv mmap))
-                       (BVal_Known (BKVal_Imm i)) en tr =
-          BVal_Unknown
-        )
-      )``,
+      (bir_number_of_mem_splits tv tr ta = NONE) ==>
+      (bir_eval_load (SOME (BVal_Mem ta tv mmap)) (SOME (BVal_Imm i)) en tr = NONE))``,
+   SIMP_TAC std_ss [bir_eval_load_NONE_REWRS])
 
-  SIMP_TAC std_ss [bir_eval_load_Unknown_REWRS]
-  );
-
-  val thm_prune1 =
-    SIMP_RULE (std_ss++bir_imm_ss++DatatypeSimps.expand_type_quants_ss [``:bir_immtype_t``, ``:bir_imm_t``])
-      [bir_number_of_mem_splits_REWRS,
-       type_of_bir_imm_def]
-      thm_prune0
+  val thm_prune1 = SIMP_RULE (std_ss ++ bir_imm_ss ++ DatatypeSimps.expand_type_quants_ss [``:bir_immtype_t``, ``:bir_imm_t``]) [bir_number_of_mem_splits_REWRS, type_of_bir_imm_def] thm_prune0
 
 
-  val (l1, l2) =
-    partition (is_imp_only o concl) (CONJUNCTS thm_prune1)
+  val (l1, l2) = partition (is_imp_only o concl) (CONJUNCTS thm_prune1)
 
-  val l1' =
-    map (
-      SIMP_RULE (list_ss++bir_imm_ss++DatatypeSimps.expand_type_quants_ss [``:bir_immtype_t``])
-      [bir_number_of_mem_splits_REWRS] o (Q.GEN `ta`)
-    ) l1
+  val l1' = map (SIMP_RULE (list_ss++bir_imm_ss++DatatypeSimps.expand_type_quants_ss [``:bir_immtype_t``]) [bir_number_of_mem_splits_REWRS] o (Q.GEN `ta`)) l1
 
-  val thm_prune2 =
-    SIMP_RULE std_ss [FORALL_AND_THM, GSYM CONJ_ASSOC]
-      (GEN_ALL (LIST_CONJ (l1' @ l2)))
+  val thm_prune2 = SIMP_RULE std_ss [FORALL_AND_THM, GSYM CONJ_ASSOC] (GEN_ALL
+    (LIST_CONJ (l1' @ l2)))
 
   val thm0 = bir_eval_load_BASIC_REWR
 
-  val thm1 =
-    SIMP_RULE (list_ss++bir_imm_ss++DatatypeSimps.expand_type_quants_ss [``:bir_immtype_t``, ``:bir_imm_t``, ``:bir_endian_t``])
-      [type_of_bir_imm_def, size_of_bir_immtype_def,
-       bir_number_of_mem_splits_REWRS, bir_load_from_mem_REWRS,
-       thm_prune2]
-      thm0
+  val thm1 = SIMP_RULE (list_ss ++ bir_imm_ss ++ DatatypeSimps.expand_type_quants_ss [``:bir_immtype_t``, ``:bir_imm_t``, ``:bir_endian_t``]) [ type_of_bir_imm_def, size_of_bir_immtype_def, bir_number_of_mem_splits_REWRS, bir_load_from_mem_REWRS, thm_prune2]
+     thm0
 
   val thm2 = Ho_Rewrite.REWRITE_RULE [fold_bir_endian_THM] thm1
 
-  val thm3 = SIMP_RULE list_ss [FORALL_AND_THM, b2n_MOD_2EXP,
-                                type_of_bir_imm_def,
-                                size_of_bir_immtype_def] thm2
+  val thm3 = SIMP_RULE (list_ss) [
+     FORALL_AND_THM, b2n_MOD_2EXP, type_of_bir_imm_def, size_of_bir_immtype_def]
+     thm2
 
-  val thm4 =
-    REWRITE_RULE [b2n_def, bir_mem_addr_w2n_SIZES,
-                  bir_mem_addr_w2n_add_SIZES, GSYM CONJ_ASSOC]
-                 (CONJ thm3 thm_prune2)
-in
-  thm4
-end
-);
+  val thm4 = REWRITE_RULE [b2n_def, bir_mem_addr_w2n_SIZES, bir_mem_addr_w2n_add_SIZES, GSYM CONJ_ASSOC] (CONJ thm3 thm_prune2)
+in thm4
+end);
 
 
 
-val bir_eval_store_Unknown_REWRS1 = prove (
-  ``(!mem en v.
-      bir_eval_store mem BVal_Unknown en v = BVal_Unknown
-    ) /\
-    (!mem en v aty vty mmap.
-      bir_eval_store mem (BVal_Known (BKVal_Mem aty vty mmap))
-                         en v = BVal_Unknown
-    )``,
+val bir_eval_store_NONE_REWRS1 = prove (
+  ``(!mem en v. bir_eval_store mem NONE en v = NONE) /\
+    (!mem en v aty vty mmap. bir_eval_store mem (SOME (BVal_Mem aty vty mmap)) en v = NONE)``,
 
 SIMP_TAC std_ss [bir_eval_store_def] >>
-REPEAT CONJ_TAC >> (
-  Cases_on `mem` >| [
-    SIMP_TAC std_ss [bir_eval_store_def],
+REPEAT CONJ_TAC >>
+Cases_on `mem` >> (TRY (Cases_on `x`)) >> SIMP_TAC std_ss [bir_eval_store_def]);
 
-    Cases_on `b` >> (
-      SIMP_TAC std_ss [bir_eval_store_def]
-    )
-  ]
-)
-);
+val bir_eval_store_NONE_REWRS2 = prove (
+  ``(!a en v. bir_eval_store NONE a en v = NONE) /\
+    (!a en v i. bir_eval_store (SOME (BVal_Imm i)) a en v = NONE)``,
 
-val bir_eval_store_Unknown_REWRS2 = prove (
-  ``(!a en v. bir_eval_store BVal_Unknown a en v = BVal_Unknown) /\
-    (!a en v i.
-      bir_eval_store (BVal_Known (BKVal_Imm i)) a en v =
-        BVal_Unknown
-    )``,
-
-SIMP_TAC std_ss [bir_eval_store_def]
-);
+SIMP_TAC std_ss [bir_eval_store_def]);
 
 
-val bir_eval_store_Unknown_REWRS3 = prove (
-  ``(!a en mem.
-      bir_eval_store mem a en BVal_Unknown = BVal_Unknown
-    ) /\
-    (!a en mem ta tv mmap.
-      bir_eval_store mem a en (BVal_Known (BKVal_Mem ta tv mmap)) =
-        BVal_Unknown
-    )``,
+val bir_eval_store_NONE_REWRS3 = prove (
+  ``(!a en mem. bir_eval_store mem a en NONE = NONE) /\
+    (!a en mem ta tv mmap. bir_eval_store mem a en (SOME (BVal_Mem ta tv mmap)) = NONE)``,
 
-REPEAT CONJ_TAC >> (
-  Cases_on `mem` >| [
-    Cases_on `a` >> (
-      SIMP_TAC std_ss [bir_eval_store_def]
-    ),
-
-    Cases_on `b` >| [
-      Cases_on `a` >> (
-	SIMP_TAC std_ss [bir_eval_store_def]
-      ),
-
-      Cases_on `a` >| [
-        SIMP_TAC std_ss [bir_eval_store_def],
-
-	Cases_on `b` >> (
-	  SIMP_TAC std_ss [bir_eval_store_def]
-	)
-      ]
-    ]
-  ]
-)
-);
+REPEAT CONJ_TAC >>
+Cases_on `mem` >> Cases_on `a` >> (TRY (Cases_on `x`)) >>
+  ((TRY (Cases_on `x'`)) >> SIMP_TAC std_ss [bir_eval_store_def]));
 
 
-val bir_eval_store_Unknown_REWRS4 = prove (
+val bir_eval_store_NONE_REWRS4 = prove (
   ``!en v i aty vty mmap.
       (type_of_bir_imm i <> aty) ==>
-      (bir_eval_store (BVal_Known (BKVal_Mem aty vty mmap))
-                      (BVal_Known (BKVal_Imm i)) en v =
-        BVal_Unknown
-      )``,
-
-Cases_on `v` >| [
-  SIMP_TAC std_ss [bir_eval_store_def],
-
-  Cases_on `b` >> (
-    SIMP_TAC std_ss [bir_eval_store_def]
-  )
-]
-);
+      (bir_eval_store (SOME (BVal_Mem aty vty mmap)) (SOME (BVal_Imm i)) en v = NONE)``,
+Cases_on `v` >> (TRY (Cases_on `x`)) >> (
+  SIMP_TAC std_ss [bir_eval_store_def]));
 
 
-val bir_eval_store_Unknown_REWRS5 = prove (
+val bir_eval_store_NONE_REWRS5 = prove (
   ``!a en v aty vty mmap.
       (type_of_bir_imm v <> vty) ==>
-      (bir_eval_store (BVal_Known (BKVal_Mem aty vty mmap)) a
-                      BEnd_NoEndian (BVal_Known (BKVal_Imm v)) =
-        BVal_Unknown
-      )``,
+      (bir_eval_store (SOME (BVal_Mem aty vty mmap)) a BEnd_NoEndian (SOME (BVal_Imm v)) = NONE)``,
 
-Cases_on `a` >| [
-  SIMP_TAC std_ss [bir_eval_store_def],
-
-  Cases_on `b` >> (
-    FULL_SIMP_TAC std_ss [bir_eval_store_def,
-                          bir_store_in_mem_NO_ENDIAN]
-  )
-]
-);
+Cases_on `a` >> SIMP_TAC std_ss [bir_eval_store_def] >>
+REPEAT STRIP_TAC >>
+Cases_on `v` >> Cases_on `vty` >> Cases_on `x` >> SIMP_TAC std_ss [bir_eval_store_def] >>
+ASM_SIMP_TAC std_ss [bir_store_in_mem_NO_ENDIAN]);
 
 
-val bir_eval_store_Unknown_REWRS6 = prove (
+val bir_eval_store_NONE_REWRS6 = prove (
   ``!a en v aty vty mmap en.
-      (bir_number_of_mem_splits vty (type_of_bir_imm v) aty =
-        NONE
-      ) ==>
-      (bir_eval_store (BVal_Known (BKVal_Mem aty vty mmap)) a en
-                      (BVal_Known (BKVal_Imm v)) = BVal_Unknown
-      )``,
+      (bir_number_of_mem_splits vty (type_of_bir_imm v) aty = NONE) ==>
+      (bir_eval_store (SOME (BVal_Mem aty vty mmap)) a en (SOME (BVal_Imm v)) = NONE)``,
 
-Cases_on `a` >| [
-  SIMP_TAC std_ss [bir_eval_store_def, LET_DEF],
-
-  Cases_on `b` >> (
-    FULL_SIMP_TAC std_ss [bir_eval_store_def,
-                          bir_store_in_mem_def, LET_DEF]
-  )
-]
-);
+Cases_on `a` >> SIMP_TAC std_ss [LET_DEF] >>
+REPEAT STRIP_TAC >>
+Cases_on `v` >> Cases_on `vty` >> TRY (Cases_on `x`) >> SIMP_TAC std_ss [bir_eval_store_def] >>
+ASM_SIMP_TAC std_ss [bir_store_in_mem_def, LET_DEF]);
 
 
-val bir_eval_store_Unknown_REWRS =
-  save_thm ("bir_eval_store_Unknown_REWRS",
+val bir_eval_store_NONE_REWRS = save_thm ("bir_eval_store_NONE_REWRS",
+  SIMP_RULE std_ss [GSYM CONJ_ASSOC] (
+  LIST_CONJ [bir_eval_store_NONE_REWRS1, bir_eval_store_NONE_REWRS2,
+             bir_eval_store_NONE_REWRS3, bir_eval_store_NONE_REWRS4,
+             bir_eval_store_NONE_REWRS5, bir_eval_store_NONE_REWRS6]));
 
-SIMP_RULE std_ss [GSYM CONJ_ASSOC] (
-  LIST_CONJ [bir_eval_store_Unknown_REWRS1,
-	     bir_eval_store_Unknown_REWRS2,
-	     bir_eval_store_Unknown_REWRS3,
-	     bir_eval_store_Unknown_REWRS4,
-	     bir_eval_store_Unknown_REWRS5,
-	     bir_eval_store_Unknown_REWRS6]
-)
-);
-
-val bir_eval_store_SINGLE_REWR =
-  store_thm ("bir_eval_store_SINGLE_REWR",
-  ``!i aty v vty mmap en.
+val bir_eval_store_SINGLE_REWR = store_thm ("bir_eval_store_SINGLE_REWR",
+  ``!a en t i aty v vty mmap en.
       ((type_of_bir_imm i = aty) /\ (type_of_bir_imm v = vty)) ==>
-      (bir_eval_store (BVal_Known (BKVal_Mem aty vty mmap))
-                      (BVal_Known (BKVal_Imm i)) en
-                      (BVal_Known (BKVal_Imm v)) =
-        BVal_Known (BKVal_Mem aty vty (FUPDATE mmap (b2n i, b2n v)))
-      )``,
+      (bir_eval_store (SOME (BVal_Mem aty vty mmap)) (SOME (BVal_Imm i)) en (SOME (BVal_Imm v)) =
+      SOME (BVal_Mem aty vty (FUPDATE mmap (b2n i, b2n v))))``,
 
 SIMP_TAC arith_ss [bir_eval_store_def, bir_store_in_mem_SINGLE] >>
 REPEAT STRIP_TAC >>
 `bir_mem_addr (type_of_bir_imm i) (b2n i) = b2n i` suffices_by ASM_SIMP_TAC std_ss [] >>
 MATCH_MP_TAC bir_mem_addr_id >>
-METIS_TAC [b2n_lt]
-);
+METIS_TAC[b2n_lt]);
 
 
-val bir_eval_store_BASIC_REWR =
-  store_thm ("bir_eval_store_BASIC_REWR",
+val bir_eval_store_BASIC_REWR = store_thm ("bir_eval_store_BASIC_REWR",
   ``!a en t i aty v vty mmap en.
-      (bir_eval_store (BVal_Known (BKVal_Mem aty vty mmap))
-                      (BVal_Known (BKVal_Imm i)) en
-                      (BVal_Known (BKVal_Imm v)) =
-        if type_of_bir_imm i = aty
-        then case bir_store_in_mem vty aty v mmap en (b2n i) of
-               NONE => BVal_Unknown
-             | SOME mmap' => BVal_Known (BKVal_Mem aty vty mmap')
-        else BVal_Unknown
-      )``,
+      (bir_eval_store (SOME (BVal_Mem aty vty mmap)) (SOME (BVal_Imm i)) en (SOME (BVal_Imm v)) =
+      (if type_of_bir_imm i = aty then
+         case bir_store_in_mem vty aty v mmap en (b2n i) of
+           NONE => NONE
+         | SOME mmap' => SOME (BVal_Mem aty vty mmap')
+       else NONE))``,
 
-SIMP_TAC arith_ss [bir_eval_store_def]
-);
+SIMP_TAC arith_ss [bir_eval_store_def]);
 
 
-val bir_eval_store_FULL_REWRS =
-  save_thm ("bir_eval_store_FULL_REWRS",
+val bir_eval_store_FULL_REWRS = save_thm ("bir_eval_store_FULL_REWRS",
 let
-  val thm_prune0 = prove (
-    ``(!ta a.
-        (type_of_bir_imm a <> ta) ==>
-        (bir_eval_store (BVal_Known (BKVal_Mem ta tv mmap))
-                        (BVal_Known (BKVal_Imm a)) en v =
-          BVal_Unknown)
-      ) /\
+  val thm_prune0 = prove (``(!ta a.
+      (type_of_bir_imm a <> ta) ==>
+      (bir_eval_store (SOME (BVal_Mem ta tv mmap)) (SOME (BVal_Imm a)) en v = NONE)) /\
       (!i tv.
-        (type_of_bir_imm i <> tv) ==>
-        (bir_number_of_mem_splits tv (type_of_bir_imm i) ta <>
-          NONE
-        ) ==>
-        (bir_eval_store (BVal_Known (BKVal_Mem ta tv mmap)) a
-                        BEnd_NoEndian (BVal_Known (BKVal_Imm i)) =
-          BVal_Unknown
-        )
-      ) /\
+      (type_of_bir_imm i <> tv) ==> (bir_number_of_mem_splits tv (type_of_bir_imm i) ta <> NONE) ==>
+      (bir_eval_store (SOME (BVal_Mem ta tv mmap)) a BEnd_NoEndian (SOME (BVal_Imm i)) = NONE)) /\
       (!i tv.
-        (bir_number_of_mem_splits tv (type_of_bir_imm i) ta =
-          NONE
-        ) ==>
-        (bir_eval_store (BVal_Known (BKVal_Mem ta tv mmap)) a en
-                        (BVal_Known (BKVal_Imm i)) =
-          BVal_Unknown
-        )
-      )``,
+      (bir_number_of_mem_splits tv (type_of_bir_imm i) ta = NONE) ==>
+      (bir_eval_store (SOME (BVal_Mem ta tv mmap)) a en (SOME (BVal_Imm i)) = NONE))``,
+   SIMP_TAC std_ss [bir_eval_store_NONE_REWRS])
 
-  SIMP_TAC std_ss [bir_eval_store_Unknown_REWRS]
-  )
+  val thm_prune1 = SIMP_RULE (std_ss ++ bir_imm_ss ++ DatatypeSimps.expand_type_quants_ss [``:bir_immtype_t``, ``:bir_imm_t``]) [bir_number_of_mem_splits_REWRS, type_of_bir_imm_def, FORALL_AND_THM] thm_prune0
 
-  val thm_prune1 =
-    SIMP_RULE (std_ss++bir_imm_ss++DatatypeSimps.expand_type_quants_ss [``:bir_immtype_t``, ``:bir_imm_t``])
-      [bir_number_of_mem_splits_REWRS, type_of_bir_imm_def,
-       FORALL_AND_THM]
-      thm_prune0
+  val (l1, l2) = partition (is_imp_only o snd o strip_forall o concl) (CONJUNCTS thm_prune1)
 
-  val (l1, l2) =
-    partition (is_imp_only o snd o strip_forall o concl)
-              (CONJUNCTS thm_prune1)
+  val l1' = map (SIMP_RULE (list_ss++bir_imm_ss++DatatypeSimps.expand_type_quants_ss [``:bir_immtype_t``]) [bir_number_of_mem_splits_REWRS] o (Q.GEN `ta`)) l1
 
-  val l1' = map (
-    SIMP_RULE (list_ss++bir_imm_ss++DatatypeSimps.expand_type_quants_ss [``:bir_immtype_t``])
-      [bir_number_of_mem_splits_REWRS] o (Q.GEN `ta`)
-  ) l1
-
-  val thm_prune2 =
-    SIMP_RULE std_ss [FORALL_AND_THM, GSYM CONJ_ASSOC]
-                     (GEN_ALL (LIST_CONJ (l1' @ l2)))
+  val thm_prune2 = SIMP_RULE std_ss [FORALL_AND_THM, GSYM CONJ_ASSOC] (GEN_ALL
+    (LIST_CONJ (l1' @ l2)))
 
 
-  val thm0 = SIMP_RULE std_ss [bir_eval_store_Unknown_REWRS,
-                               FORALL_AND_THM]
-                              bir_eval_store_BASIC_REWR
+  val thm0 = SIMP_RULE (std_ss) [bir_eval_store_NONE_REWRS, FORALL_AND_THM] bir_eval_store_BASIC_REWR
 
-  val thm1 =
-    SIMP_RULE (list_ss++bir_imm_ss++DatatypeSimps.expand_type_quants_ss [``:bir_immtype_t``, ``:bir_imm_t``, ``:bir_endian_t``])
-      [type_of_bir_imm_def, size_of_bir_immtype_def,
-       bir_number_of_mem_splits_REWRS, bir_store_in_mem_REWRS,
-       thm_prune2] thm0
+  val thm1 = SIMP_RULE (list_ss++ bir_imm_ss ++ DatatypeSimps.expand_type_quants_ss [``:bir_immtype_t``, ``:bir_imm_t``, ``:bir_endian_t``]) [ type_of_bir_imm_def, size_of_bir_immtype_def, bir_number_of_mem_splits_REWRS, bir_store_in_mem_REWRS, thm_prune2]
+     thm0
 
   val thm2 = Ho_Rewrite.REWRITE_RULE [fold_bir_endian_THM] thm1
 
-  val thm3 =
-    SIMP_RULE list_ss [FORALL_AND_THM, type_of_bir_imm_def,
-                       size_of_bir_immtype_def] thm2
+  val thm3 = SIMP_RULE (list_ss) [
+     FORALL_AND_THM, type_of_bir_imm_def, size_of_bir_immtype_def]
+     thm2
 
-  val thm4 =
-    REWRITE_RULE [b2n_def, GSYM CONJ_ASSOC] (CONJ thm3 thm_prune2)
-in
-  thm4
-end
-);
+  val thm4 = REWRITE_RULE [b2n_def, GSYM CONJ_ASSOC] (CONJ thm3 thm_prune2)
+in thm4
+end);
 
 
 val _ = export_theory();
